Regoose; defn and theory for interfaces; fix proofs to use sync.Locker
interface for sync.Cond

new/golang/defn/interface.v
@@ -1,14 +1,24 @@
 From Perennial.goose_lang Require Import notation.
+From New.golang.defn Require Import struct typing.
 
 Module interface.
 Section goose_lang.
 Context `{ffi_syntax}.
+Local Coercion Var' (s:string) : expr := Var s.
 
-Definition call : val.
-Admitted.
+Definition get (f : string) : val :=
+  λ: "v", let: (("typeid", "val"), "mset") := "v" in
+          let: "mset" := (match: "mset" with InjL "v" => "v" | InjR <> => Panic "interface" end) in
+          (match: (struct.assocl_lookup #(str f) "mset") with
+            InjL <> => #()
+            | InjR "m" => "m"
+          end) (match: "val" with InjL "v" => "v" | InjR <> => Panic "interface" end)
+.
 
-Definition val (x : gmap string val) : val.
-Admitted.
+Local Definition make_def (mset : list (string*val)) : val :=
+  λ: "v", (#(str "NO TYPE IDS YET"), InjL "v", InjL (struct.fields_val mset)).
+Program Definition make := unseal (_:seal (@make_def)). Obligation 1. by eexists. Qed.
+Definition make_unseal : make = _ := seal_eq _.
 
 End goose_lang.
 End interface.
