new/code/github_com/mit_pdos/gokv/urpc.v
@@ -13,6 +13,10 @@ Definition Server : go_type := structT [
   "handlers" :: mapT uint64T funcT
 ].
 
+Definition Server__mset : list (string * val) := [
+].
+
+(* go: urpc.go:19:20 *)
 Definition Server__rpcHandle : val :=
   rec: "Server__rpcHandle" "srv" "conn" "rpcid" "seqno" "data" :=
     exception_do (let: "srv" := ref_ty ptrT "srv" in
@@ -21,89 +25,120 @@ Definition Server__rpcHandle : val :=
     let: "rpcid" := ref_ty uint64T "rpcid" in
     let: "conn" := ref_ty grove_ffi.Connection "conn" in
     let: "replyData" := ref_ty ptrT (zero_val ptrT) in
-    let: "$a0" := ref_ty (sliceT byteT) (zero_val (sliceT byteT)) in
-    do:  "replyData" <-[ptrT] "$a0";;;
+    let: "$r0" := ref_ty (sliceT byteT) (zero_val (sliceT byteT)) in
+    do:  ("replyData" <-[ptrT] "$r0");;;
     let: "f" := ref_ty funcT (zero_val funcT) in
-    let: "$a0" := Fst (map.get (![mapT uint64T funcT] (struct.field_ref Server "handlers" (![ptrT] "srv"))) (![uint64T] "rpcid")) in
-    do:  "f" <-[funcT] "$a0";;;
-    do:  (![funcT] "f") (![sliceT byteT] "data") (![ptrT] "replyData");;;
+    let: "$r0" := Fst (map.get (![mapT uint64T funcT] (struct.field_ref Server "handlers" (![ptrT] "srv"))) (![uint64T] "rpcid")) in
+    do:  ("f" <-[funcT] "$r0");;;
+    do:  (let: "$a0" := ![sliceT byteT] "data" in
+    let: "$a1" := ![ptrT] "replyData" in
+    (![funcT] "f") "$a0" "$a1");;;
     let: "data1" := ref_ty (sliceT byteT) (zero_val (sliceT byteT)) in
-    let: "$a0" := slice.make3 byteT #0 (#8 + (slice.len (![sliceT byteT] (![ptrT] "replyData")))) in
-    do:  "data1" <-[sliceT byteT] "$a0";;;
+    let: "$r0" := slice.make3 byteT #0 (#8 + (slice.len (![sliceT byteT] (![ptrT] "replyData")))) in
+    do:  ("data1" <-[sliceT byteT] "$r0");;;
     let: "data2" := ref_ty (sliceT byteT) (zero_val (sliceT byteT)) in
-    let: "$a0" := marshal.WriteInt (![sliceT byteT] "data1") (![uint64T] "seqno") in
-    do:  "data2" <-[sliceT byteT] "$a0";;;
+    let: "$r0" := let: "$a0" := ![sliceT byteT] "data1" in
+    let: "$a1" := ![uint64T] "seqno" in
+    marshal.WriteInt "$a0" "$a1" in
+    do:  ("data2" <-[sliceT byteT] "$r0");;;
     let: "data3" := ref_ty (sliceT byteT) (zero_val (sliceT byteT)) in
-    let: "$a0" := marshal.WriteBytes (![sliceT byteT] "data2") (![sliceT byteT] (![ptrT] "replyData")) in
-    do:  "data3" <-[sliceT byteT] "$a0";;;
-    do:  grove_ffi.Send (![grove_ffi.Connection] "conn") (![sliceT byteT] "data3");;;
+    let: "$r0" := let: "$a0" := ![sliceT byteT] "data2" in
+    let: "$a1" := ![sliceT byteT] (![ptrT] "replyData") in
+    marshal.WriteBytes "$a0" "$a1" in
+    do:  ("data3" <-[sliceT byteT] "$r0");;;
+    do:  (let: "$a0" := ![grove_ffi.Connection] "conn" in
+    let: "$a1" := ![sliceT byteT] "data3" in
+    grove_ffi.Send "$a0" "$a1");;;
     do:  #()).
 
-Definition MakeServer : val :=
-  rec: "MakeServer" "handlers" :=
-    exception_do (let: "handlers" := ref_ty (mapT uint64T funcT) "handlers" in
-    return: (ref_ty Server (struct.make Server [{
-       "handlers" ::= ![mapT uint64T funcT] "handlers"
-     }]));;;
-    do:  #()).
-
+(* go: urpc.go:36:20 *)
 Definition Server__readThread : val :=
   rec: "Server__readThread" "srv" "conn" :=
     exception_do (let: "srv" := ref_ty ptrT "srv" in
     let: "conn" := ref_ty grove_ffi.Connection "conn" in
     (for: (λ: <>, #true); (λ: <>, Skip) := λ: <>,
       let: "r" := ref_ty grove_ffi.ReceiveRet (zero_val grove_ffi.ReceiveRet) in
-      let: "$a0" := grove_ffi.Receive (![grove_ffi.Connection] "conn") in
-      do:  "r" <-[grove_ffi.ReceiveRet] "$a0";;;
+      let: "$r0" := let: "$a0" := ![grove_ffi.Connection] "conn" in
+      grove_ffi.Receive "$a0" in
+      do:  ("r" <-[grove_ffi.ReceiveRet] "$r0");;;
       (if: ![boolT] (struct.field_ref grove_ffi.ReceiveRet "Err" "r")
       then
         break: #();;;
         do:  #()
       else do:  #());;;
       let: "data" := ref_ty (sliceT byteT) (zero_val (sliceT byteT)) in
-      let: "$a0" := ![sliceT byteT] (struct.field_ref grove_ffi.ReceiveRet "Data" "r") in
-      do:  "data" <-[sliceT byteT] "$a0";;;
+      let: "$r0" := ![sliceT byteT] (struct.field_ref grove_ffi.ReceiveRet "Data" "r") in
+      do:  ("data" <-[sliceT byteT] "$r0");;;
       let: "rpcid" := ref_ty uint64T (zero_val uint64T) in
-      let: ("$a0", "$a1") := marshal.ReadInt (![sliceT byteT] "data") in
-      do:  "data" <-[sliceT byteT] "$a1";;;
-      do:  "rpcid" <-[uint64T] "$a0";;;
+      let: ("$ret0", "$ret1") := let: "$a0" := ![sliceT byteT] "data" in
+      marshal.ReadInt "$a0" in
+      let: "$r0" := "$ret0" in
+      let: "$r1" := "$ret1" in
+      do:  ("rpcid" <-[uint64T] "$r0");;;
+      do:  ("data" <-[sliceT byteT] "$r1");;;
       let: "seqno" := ref_ty uint64T (zero_val uint64T) in
-      let: ("$a0", "$a1") := marshal.ReadInt (![sliceT byteT] "data") in
-      do:  "data" <-[sliceT byteT] "$a1";;;
-      do:  "seqno" <-[uint64T] "$a0";;;
+      let: ("$ret0", "$ret1") := let: "$a0" := ![sliceT byteT] "data" in
+      marshal.ReadInt "$a0" in
+      let: "$r0" := "$ret0" in
+      let: "$r1" := "$ret1" in
+      do:  ("seqno" <-[uint64T] "$r0");;;
+      do:  ("data" <-[sliceT byteT] "$r1");;;
       let: "req" := ref_ty (sliceT byteT) (zero_val (sliceT byteT)) in
-      let: "$a0" := ![sliceT byteT] "data" in
-      do:  "req" <-[sliceT byteT] "$a0";;;
+      let: "$r0" := ![sliceT byteT] "data" in
+      do:  ("req" <-[sliceT byteT] "$r0");;;
       let: "$go" := (λ: <>,
-        do:  (Server__rpcHandle (![ptrT] "srv")) (![grove_ffi.Connection] "conn") (![uint64T] "rpcid") (![uint64T] "seqno") (![sliceT byteT] "req");;;
+        do:  (let: "$a0" := ![grove_ffi.Connection] "conn" in
+        let: "$a1" := ![uint64T] "rpcid" in
+        let: "$a2" := ![uint64T] "seqno" in
+        let: "$a3" := ![sliceT byteT] "req" in
+        (Server__rpcHandle (![ptrT] "srv")) "$a0" "$a1" "$a2" "$a3");;;
         do:  #()
         ) in
-      do:  Fork ("$go" #());;;
+      do:  (Fork ("$go" #()));;;
       continue: #();;;
       do:  #());;;
     do:  #()).
 
+(* go: urpc.go:58:20 *)
 Definition Server__Serve : val :=
   rec: "Server__Serve" "srv" "host" :=
     exception_do (let: "srv" := ref_ty ptrT "srv" in
     let: "host" := ref_ty uint64T "host" in
     let: "listener" := ref_ty grove_ffi.Listener (zero_val grove_ffi.Listener) in
-    let: "$a0" := grove_ffi.Listen (![uint64T] "host") in
-    do:  "listener" <-[grove_ffi.Listener] "$a0";;;
+    let: "$r0" := let: "$a0" := ![uint64T] "host" in
+    grove_ffi.Listen "$a0" in
+    do:  ("listener" <-[grove_ffi.Listener] "$r0");;;
     let: "$go" := (λ: <>,
       (for: (λ: <>, #true); (λ: <>, Skip) := λ: <>,
         let: "conn" := ref_ty grove_ffi.Connection (zero_val grove_ffi.Connection) in
-        let: "$a0" := grove_ffi.Accept (![grove_ffi.Listener] "listener") in
-        do:  "conn" <-[grove_ffi.Connection] "$a0";;;
+        let: "$r0" := let: "$a0" := ![grove_ffi.Listener] "listener" in
+        grove_ffi.Accept "$a0" in
+        do:  ("conn" <-[grove_ffi.Connection] "$r0");;;
         let: "$go" := (λ: <>,
-          do:  (Server__readThread (![ptrT] "srv")) (![grove_ffi.Connection] "conn");;;
+          do:  (let: "$a0" := ![grove_ffi.Connection] "conn" in
+          (Server__readThread (![ptrT] "srv")) "$a0");;;
           do:  #()
           ) in
-        do:  Fork ("$go" #());;;
+        do:  (Fork ("$go" #()));;;
         do:  #());;;
       do:  #()
       ) in
-    do:  Fork ("$go" #());;;
+    do:  (Fork ("$go" #()));;;
+    do:  #()).
+
+Definition Server__mset_ptr : list (string * val) := [
+  ("Serve", Server__Serve);
+  ("readThread", Server__readThread);
+  ("rpcHandle", Server__rpcHandle)
+].
+
+(* go: urpc.go:32:6 *)
+Definition MakeServer : val :=
+  rec: "MakeServer" "handlers" :=
+    exception_do (let: "handlers" := ref_ty (mapT uint64T funcT) "handlers" in
+    return: (ref_ty Server (struct.make Server [{
+       "handlers" ::= ![mapT uint64T funcT] "handlers"
+     }]));;;
     do:  #()).
 
 Definition callbackStateWaiting : expr := #0.
@@ -118,6 +153,12 @@ Definition Callback : go_type := structT [
   "cond" :: ptrT
 ].
 
+Definition Callback__mset : list (string * val) := [
+].
+
+Definition Callback__mset_ptr : list (string * val) := [
+].
+
 Definition Client : go_type := structT [
   "mu" :: ptrT;
   "conn" :: grove_ffi.Connection;
@@ -125,183 +166,40 @@ Definition Client : go_type := structT [
   "pending" :: mapT uint64T ptrT
 ].
 
-Definition Client__replyThread : val :=
-  rec: "Client__replyThread" "cl" <> :=
-    exception_do (let: "cl" := ref_ty ptrT "cl" in
-    (for: (λ: <>, #true); (λ: <>, Skip) := λ: <>,
-      let: "r" := ref_ty grove_ffi.ReceiveRet (zero_val grove_ffi.ReceiveRet) in
-      let: "$a0" := grove_ffi.Receive (![grove_ffi.Connection] (struct.field_ref Client "conn" (![ptrT] "cl"))) in
-      do:  "r" <-[grove_ffi.ReceiveRet] "$a0";;;
-      (if: ![boolT] (struct.field_ref grove_ffi.ReceiveRet "Err" "r")
-      then
-        do:  (sync.Mutex__Lock (![ptrT] (struct.field_ref Client "mu" (![ptrT] "cl")))) #();;;
-        do:  MapIter (![mapT uint64T ptrT] (struct.field_ref Client "pending" (![ptrT] "cl"))) (λ: <> "cb",
-          let: "$a0" := callbackStateAborted in
-          do:  (![ptrT] (struct.field_ref Callback "state" (![ptrT] "cb"))) <-[uint64T] "$a0";;;
-          do:  (sync.Cond__Signal (![ptrT] (struct.field_ref Callback "cond" (![ptrT] "cb")))) #();;;
-          do:  #());;;
-        do:  (sync.Mutex__Unlock (![ptrT] (struct.field_ref Client "mu" (![ptrT] "cl")))) #();;;
-        break: #();;;
-        do:  #()
-      else do:  #());;;
-      let: "data" := ref_ty (sliceT byteT) (zero_val (sliceT byteT)) in
-      let: "$a0" := ![sliceT byteT] (struct.field_ref grove_ffi.ReceiveRet "Data" "r") in
-      do:  "data" <-[sliceT byteT] "$a0";;;
-      let: "seqno" := ref_ty uint64T (zero_val uint64T) in
-      let: ("$a0", "$a1") := marshal.ReadInt (![sliceT byteT] "data") in
-      do:  "data" <-[sliceT byteT] "$a1";;;
-      do:  "seqno" <-[uint64T] "$a0";;;
-      let: "reply" := ref_ty (sliceT byteT) (zero_val (sliceT byteT)) in
-      let: "$a0" := ![sliceT byteT] "data" in
-      do:  "reply" <-[sliceT byteT] "$a0";;;
-      do:  (sync.Mutex__Lock (![ptrT] (struct.field_ref Client "mu" (![ptrT] "cl")))) #();;;
-      let: "ok" := ref_ty boolT (zero_val boolT) in
-      let: "cb" := ref_ty ptrT (zero_val ptrT) in
-      let: ("$a0", "$a1") := Fst (map.get (![mapT uint64T ptrT] (struct.field_ref Client "pending" (![ptrT] "cl"))) (![uint64T] "seqno")) in
-      do:  "ok" <-[boolT] "$a1";;;
-      do:  "cb" <-[ptrT] "$a0";;;
-      (if: ![boolT] "ok"
-      then
-        do:  MapDelete (![mapT uint64T ptrT] (struct.field_ref Client "pending" (![ptrT] "cl"))) (![uint64T] "seqno");;;
-        let: "$a0" := ![sliceT byteT] "reply" in
-        do:  (![ptrT] (struct.field_ref Callback "reply" (![ptrT] "cb"))) <-[sliceT byteT] "$a0";;;
-        let: "$a0" := callbackStateDone in
-        do:  (![ptrT] (struct.field_ref Callback "state" (![ptrT] "cb"))) <-[uint64T] "$a0";;;
-        do:  (sync.Cond__Signal (![ptrT] (struct.field_ref Callback "cond" (![ptrT] "cb")))) #();;;
-        do:  #()
-      else do:  #());;;
-      do:  (sync.Mutex__Unlock (![ptrT] (struct.field_ref Client "mu" (![ptrT] "cl")))) #();;;
-      continue: #();;;
-      do:  #());;;
-    do:  #()).
-
-Definition TryMakeClient : val :=
-  rec: "TryMakeClient" "host_name" :=
-    exception_do (let: "host_name" := ref_ty uint64T "host_name" in
-    let: "host" := ref_ty uint64T (zero_val uint64T) in
-    let: "$a0" := ![uint64T] "host_name" in
-    do:  "host" <-[uint64T] "$a0";;;
-    let: "a" := ref_ty grove_ffi.ConnectRet (zero_val grove_ffi.ConnectRet) in
-    let: "$a0" := grove_ffi.Connect (![uint64T] "host") in
-    do:  "a" <-[grove_ffi.ConnectRet] "$a0";;;
-    let: "nilClient" := ref_ty ptrT (zero_val ptrT) in
-    (if: ![boolT] (struct.field_ref grove_ffi.ConnectRet "Err" "a")
-    then
-      return: (#1, ![ptrT] "nilClient");;;
-      do:  #()
-    else do:  #());;;
-    let: "cl" := ref_ty ptrT (zero_val ptrT) in
-    let: "$a0" := ref_ty Client (struct.make Client [{
-      "conn" ::= ![grove_ffi.Connection] (struct.field_ref grove_ffi.ConnectRet "Connection" "a");
-      "mu" ::= ref_ty sync.Mutex (zero_val sync.Mutex);
-      "seq" ::= #1;
-      "pending" ::= map.make uint64T ptrT #()
-    }]) in
-    do:  "cl" <-[ptrT] "$a0";;;
-    let: "$go" := (λ: <>,
-      do:  (Client__replyThread (![ptrT] "cl")) #();;;
-      do:  #()
-      ) in
-    do:  Fork ("$go" #());;;
-    return: (#0, ![ptrT] "cl");;;
-    do:  #()).
-
-Definition MakeClient : val :=
-  rec: "MakeClient" "host_name" :=
-    exception_do (let: "host_name" := ref_ty uint64T "host_name" in
-    let: "cl" := ref_ty ptrT (zero_val ptrT) in
-    let: "err" := ref_ty uint64T (zero_val uint64T) in
-    let: ("$a0", "$a1") := TryMakeClient (![uint64T] "host_name") in
-    do:  "cl" <-[ptrT] "$a1";;;
-    do:  "err" <-[uint64T] "$a0";;;
-    (if: (![uint64T] "err") ≠ #0
-    then
-      do:  log.Printf #(str "Unable to connect to %!!(MISSING)!(MISSING)!(MISSING)!(MISSING)!(MISSING)s(MISSING)") (grove_ffi.AddressToStr (![uint64T] "host_name"));;;
-      do:  #()
-    else do:  #());;;
-    do:  machine.Assume ((![uint64T] "err") = #0);;;
-    return: (![ptrT] "cl");;;
-    do:  #()).
-
-Definition Error : go_type := uint64T.
-
-Definition ErrNone : expr := #0.
+Definition Client__mset : list (string * val) := [
+].
 
 Definition ErrTimeout : expr := #1.
 
 Definition ErrDisconnect : expr := #2.
 
-Definition Client__CallStart : val :=
-  rec: "Client__CallStart" "cl" "rpcid" "args" :=
-    exception_do (let: "cl" := ref_ty ptrT "cl" in
-    let: "args" := ref_ty (sliceT byteT) "args" in
-    let: "rpcid" := ref_ty uint64T "rpcid" in
-    let: "reply_buf" := ref_ty ptrT (zero_val ptrT) in
-    let: "$a0" := ref_ty (sliceT byteT) (zero_val (sliceT byteT)) in
-    do:  "reply_buf" <-[ptrT] "$a0";;;
-    let: "cb" := ref_ty ptrT (zero_val ptrT) in
-    let: "$a0" := ref_ty Callback (struct.make Callback [{
-      "reply" ::= ![ptrT] "reply_buf";
-      "state" ::= ref_ty uint64T (zero_val uint64T);
-      "cond" ::= sync.NewCond (![ptrT] (struct.field_ref Client "mu" (![ptrT] "cl")))
-    }]) in
-    do:  "cb" <-[ptrT] "$a0";;;
-    let: "$a0" := callbackStateWaiting in
-    do:  (![ptrT] (struct.field_ref Callback "state" (![ptrT] "cb"))) <-[uint64T] "$a0";;;
-    do:  (sync.Mutex__Lock (![ptrT] (struct.field_ref Client "mu" (![ptrT] "cl")))) #();;;
-    let: "seqno" := ref_ty uint64T (zero_val uint64T) in
-    let: "$a0" := ![uint64T] (struct.field_ref Client "seq" (![ptrT] "cl")) in
-    do:  "seqno" <-[uint64T] "$a0";;;
-    let: "$a0" := std.SumAssumeNoOverflow (![uint64T] (struct.field_ref Client "seq" (![ptrT] "cl"))) #1 in
-    do:  (struct.field_ref Client "seq" (![ptrT] "cl")) <-[uint64T] "$a0";;;
-    let: "$a0" := ![ptrT] "cb" in
-    do:  map.insert (![mapT uint64T ptrT] (struct.field_ref Client "pending" (![ptrT] "cl"))) (![uint64T] "seqno") "$a0";;;
-    do:  (sync.Mutex__Unlock (![ptrT] (struct.field_ref Client "mu" (![ptrT] "cl")))) #();;;
-    let: "data1" := ref_ty (sliceT byteT) (zero_val (sliceT byteT)) in
-    let: "$a0" := slice.make3 byteT #0 ((#8 + #8) + (slice.len (![sliceT byteT] "args"))) in
-    do:  "data1" <-[sliceT byteT] "$a0";;;
-    let: "data2" := ref_ty (sliceT byteT) (zero_val (sliceT byteT)) in
-    let: "$a0" := marshal.WriteInt (![sliceT byteT] "data1") (![uint64T] "rpcid") in
-    do:  "data2" <-[sliceT byteT] "$a0";;;
-    let: "data3" := ref_ty (sliceT byteT) (zero_val (sliceT byteT)) in
-    let: "$a0" := marshal.WriteInt (![sliceT byteT] "data2") (![uint64T] "seqno") in
-    do:  "data3" <-[sliceT byteT] "$a0";;;
-    let: "reqData" := ref_ty (sliceT byteT) (zero_val (sliceT byteT)) in
-    let: "$a0" := marshal.WriteBytes (![sliceT byteT] "data3") (![sliceT byteT] "args") in
-    do:  "reqData" <-[sliceT byteT] "$a0";;;
-    (if: grove_ffi.Send (![grove_ffi.Connection] (struct.field_ref Client "conn" (![ptrT] "cl"))) (![sliceT byteT] "reqData")
-    then
-      return: (ref_ty Callback (struct.make Callback [{
-       }]), ErrDisconnect);;;
-      do:  #()
-    else do:  #());;;
-    return: (![ptrT] "cb", ErrNone);;;
-    do:  #()).
-
+(* go: urpc.go:188:19 *)
 Definition Client__CallComplete : val :=
   rec: "Client__CallComplete" "cl" "cb" "reply" "timeout_ms" :=
     exception_do (let: "cl" := ref_ty ptrT "cl" in
     let: "timeout_ms" := ref_ty uint64T "timeout_ms" in
     let: "reply" := ref_ty ptrT "reply" in
     let: "cb" := ref_ty ptrT "cb" in
-    do:  (sync.Mutex__Lock (![ptrT] (struct.field_ref Client "mu" (![ptrT] "cl")))) #();;;
+    do:  ((sync.Mutex__Lock (![ptrT] (struct.field_ref Client "mu" (![ptrT] "cl")))) #());;;
     (if: (![uint64T] (![ptrT] (struct.field_ref Callback "state" (![ptrT] "cb")))) = callbackStateWaiting
     then
-      do:  machine.WaitTimeout (![ptrT] (struct.field_ref Callback "cond" (![ptrT] "cb"))) (![uint64T] "timeout_ms");;;
+      do:  (let: "$a0" := ![ptrT] (struct.field_ref Callback "cond" (![ptrT] "cb")) in
+      let: "$a1" := ![uint64T] "timeout_ms" in
+      machine.WaitTimeout "$a0" "$a1");;;
       do:  #()
     else do:  #());;;
     let: "state" := ref_ty uint64T (zero_val uint64T) in
-    let: "$a0" := ![uint64T] (![ptrT] (struct.field_ref Callback "state" (![ptrT] "cb"))) in
-    do:  "state" <-[uint64T] "$a0";;;
+    let: "$r0" := ![uint64T] (![ptrT] (struct.field_ref Callback "state" (![ptrT] "cb"))) in
+    do:  ("state" <-[uint64T] "$r0");;;
     (if: (![uint64T] "state") = callbackStateDone
     then
-      let: "$a0" := ![sliceT byteT] (![ptrT] (struct.field_ref Callback "reply" (![ptrT] "cb"))) in
-      do:  (![ptrT] "reply") <-[sliceT byteT] "$a0";;;
-      do:  (sync.Mutex__Unlock (![ptrT] (struct.field_ref Client "mu" (![ptrT] "cl")))) #();;;
+      let: "$r0" := ![sliceT byteT] (![ptrT] (struct.field_ref Callback "reply" (![ptrT] "cb"))) in
+      do:  ((![ptrT] "reply") <-[sliceT byteT] "$r0");;;
+      do:  ((sync.Mutex__Unlock (![ptrT] (struct.field_ref Client "mu" (![ptrT] "cl")))) #());;;
       return: (#0);;;
       do:  #()
     else
-      do:  (sync.Mutex__Unlock (![ptrT] (struct.field_ref Client "mu" (![ptrT] "cl")))) #();;;
+      do:  ((sync.Mutex__Unlock (![ptrT] (struct.field_ref Client "mu" (![ptrT] "cl")))) #());;;
       (if: (![uint64T] "state") = callbackStateAborted
       then
         return: (ErrDisconnect);;;
@@ -312,6 +210,68 @@ Definition Client__CallComplete : val :=
       do:  #());;;
     do:  #()).
 
+Definition ErrNone : expr := #0.
+
+(* go: urpc.go:155:19 *)
+Definition Client__CallStart : val :=
+  rec: "Client__CallStart" "cl" "rpcid" "args" :=
+    exception_do (let: "cl" := ref_ty ptrT "cl" in
+    let: "args" := ref_ty (sliceT byteT) "args" in
+    let: "rpcid" := ref_ty uint64T "rpcid" in
+    let: "reply_buf" := ref_ty ptrT (zero_val ptrT) in
+    let: "$r0" := ref_ty (sliceT byteT) (zero_val (sliceT byteT)) in
+    do:  ("reply_buf" <-[ptrT] "$r0");;;
+    let: "cb" := ref_ty ptrT (zero_val ptrT) in
+    let: "$r0" := ref_ty Callback (struct.make Callback [{
+      "reply" ::= ![ptrT] "reply_buf";
+      "state" ::= ref_ty uint64T (zero_val uint64T);
+      "cond" ::= let: "$a0" := interface.make sync.Mutex__mset_ptr (![ptrT] (struct.field_ref Client "mu" (![ptrT] "cl"))) in
+      sync.NewCond "$a0"
+    }]) in
+    do:  ("cb" <-[ptrT] "$r0");;;
+    let: "$r0" := callbackStateWaiting in
+    do:  ((![ptrT] (struct.field_ref Callback "state" (![ptrT] "cb"))) <-[uint64T] "$r0");;;
+    do:  ((sync.Mutex__Lock (![ptrT] (struct.field_ref Client "mu" (![ptrT] "cl")))) #());;;
+    let: "seqno" := ref_ty uint64T (zero_val uint64T) in
+    let: "$r0" := ![uint64T] (struct.field_ref Client "seq" (![ptrT] "cl")) in
+    do:  ("seqno" <-[uint64T] "$r0");;;
+    let: "$r0" := let: "$a0" := ![uint64T] (struct.field_ref Client "seq" (![ptrT] "cl")) in
+    let: "$a1" := #1 in
+    std.SumAssumeNoOverflow "$a0" "$a1" in
+    do:  ((struct.field_ref Client "seq" (![ptrT] "cl")) <-[uint64T] "$r0");;;
+    let: "$r0" := ![ptrT] "cb" in
+    do:  (map.insert (![mapT uint64T ptrT] (struct.field_ref Client "pending" (![ptrT] "cl"))) (![uint64T] "seqno") "$r0");;;
+    do:  ((sync.Mutex__Unlock (![ptrT] (struct.field_ref Client "mu" (![ptrT] "cl")))) #());;;
+    let: "data1" := ref_ty (sliceT byteT) (zero_val (sliceT byteT)) in
+    let: "$r0" := slice.make3 byteT #0 ((#8 + #8) + (slice.len (![sliceT byteT] "args"))) in
+    do:  ("data1" <-[sliceT byteT] "$r0");;;
+    let: "data2" := ref_ty (sliceT byteT) (zero_val (sliceT byteT)) in
+    let: "$r0" := let: "$a0" := ![sliceT byteT] "data1" in
+    let: "$a1" := ![uint64T] "rpcid" in
+    marshal.WriteInt "$a0" "$a1" in
+    do:  ("data2" <-[sliceT byteT] "$r0");;;
+    let: "data3" := ref_ty (sliceT byteT) (zero_val (sliceT byteT)) in
+    let: "$r0" := let: "$a0" := ![sliceT byteT] "data2" in
+    let: "$a1" := ![uint64T] "seqno" in
+    marshal.WriteInt "$a0" "$a1" in
+    do:  ("data3" <-[sliceT byteT] "$r0");;;
+    let: "reqData" := ref_ty (sliceT byteT) (zero_val (sliceT byteT)) in
+    let: "$r0" := let: "$a0" := ![sliceT byteT] "data3" in
+    let: "$a1" := ![sliceT byteT] "args" in
+    marshal.WriteBytes "$a0" "$a1" in
+    do:  ("reqData" <-[sliceT byteT] "$r0");;;
+    (if: let: "$a0" := ![grove_ffi.Connection] (struct.field_ref Client "conn" (![ptrT] "cl")) in
+    let: "$a1" := ![sliceT byteT] "reqData" in
+    grove_ffi.Send "$a0" "$a1"
+    then
+      return: (ref_ty Callback (struct.make Callback [{
+       }]), ErrDisconnect);;;
+      do:  #()
+    else do:  #());;;
+    return: (![ptrT] "cb", ErrNone);;;
+    do:  #()).
+
+(* go: urpc.go:215:19 *)
 Definition Client__Call : val :=
   rec: "Client__Call" "cl" "rpcid" "args" "reply" "timeout_ms" :=
     exception_do (let: "cl" := ref_ty ptrT "cl" in
@@ -321,13 +281,145 @@ Definition Client__Call : val :=
     let: "rpcid" := ref_ty uint64T "rpcid" in
     let: "err" := ref_ty uint64T (zero_val uint64T) in
     let: "cb" := ref_ty ptrT (zero_val ptrT) in
-    let: ("$a0", "$a1") := (Client__CallStart (![ptrT] "cl")) (![uint64T] "rpcid") (![sliceT byteT] "args") in
-    do:  "err" <-[uint64T] "$a1";;;
-    do:  "cb" <-[ptrT] "$a0";;;
+    let: ("$ret0", "$ret1") := let: "$a0" := ![uint64T] "rpcid" in
+    let: "$a1" := ![sliceT byteT] "args" in
+    (Client__CallStart (![ptrT] "cl")) "$a0" "$a1" in
+    let: "$r0" := "$ret0" in
+    let: "$r1" := "$ret1" in
+    do:  ("cb" <-[ptrT] "$r0");;;
+    do:  ("err" <-[uint64T] "$r1");;;
     (if: (![uint64T] "err") ≠ #0
     then
       return: (![uint64T] "err");;;
       do:  #()
     else do:  #());;;
-    return: ((Client__CallComplete (![ptrT] "cl")) (![ptrT] "cb") (![ptrT] "reply") (![uint64T] "timeout_ms"));;;
+    return: (let: "$a0" := ![ptrT] "cb" in
+     let: "$a1" := ![ptrT] "reply" in
+     let: "$a2" := ![uint64T] "timeout_ms" in
+     (Client__CallComplete (![ptrT] "cl")) "$a0" "$a1" "$a2");;;
     do:  #()).
+
+(* go: urpc.go:88:19 *)
+Definition Client__replyThread : val :=
+  rec: "Client__replyThread" "cl" <> :=
+    exception_do (let: "cl" := ref_ty ptrT "cl" in
+    (for: (λ: <>, #true); (λ: <>, Skip) := λ: <>,
+      let: "r" := ref_ty grove_ffi.ReceiveRet (zero_val grove_ffi.ReceiveRet) in
+      let: "$r0" := let: "$a0" := ![grove_ffi.Connection] (struct.field_ref Client "conn" (![ptrT] "cl")) in
+      grove_ffi.Receive "$a0" in
+      do:  ("r" <-[grove_ffi.ReceiveRet] "$r0");;;
+      (if: ![boolT] (struct.field_ref grove_ffi.ReceiveRet "Err" "r")
+      then
+        do:  ((sync.Mutex__Lock (![ptrT] (struct.field_ref Client "mu" (![ptrT] "cl")))) #());;;
+        do:  (MapIter (![mapT uint64T ptrT] (struct.field_ref Client "pending" (![ptrT] "cl"))) (λ: <> "cb",
+          let: "$r0" := callbackStateAborted in
+          do:  ((![ptrT] (struct.field_ref Callback "state" (![ptrT] "cb"))) <-[uint64T] "$r0");;;
+          do:  ((sync.Cond__Signal (![ptrT] (struct.field_ref Callback "cond" (![ptrT] "cb")))) #());;;
+          do:  #()));;;
+        do:  ((sync.Mutex__Unlock (![ptrT] (struct.field_ref Client "mu" (![ptrT] "cl")))) #());;;
+        break: #();;;
+        do:  #()
+      else do:  #());;;
+      let: "data" := ref_ty (sliceT byteT) (zero_val (sliceT byteT)) in
+      let: "$r0" := ![sliceT byteT] (struct.field_ref grove_ffi.ReceiveRet "Data" "r") in
+      do:  ("data" <-[sliceT byteT] "$r0");;;
+      let: "seqno" := ref_ty uint64T (zero_val uint64T) in
+      let: ("$ret0", "$ret1") := let: "$a0" := ![sliceT byteT] "data" in
+      marshal.ReadInt "$a0" in
+      let: "$r0" := "$ret0" in
+      let: "$r1" := "$ret1" in
+      do:  ("seqno" <-[uint64T] "$r0");;;
+      do:  ("data" <-[sliceT byteT] "$r1");;;
+      let: "reply" := ref_ty (sliceT byteT) (zero_val (sliceT byteT)) in
+      let: "$r0" := ![sliceT byteT] "data" in
+      do:  ("reply" <-[sliceT byteT] "$r0");;;
+      do:  ((sync.Mutex__Lock (![ptrT] (struct.field_ref Client "mu" (![ptrT] "cl")))) #());;;
+      let: "ok" := ref_ty boolT (zero_val boolT) in
+      let: "cb" := ref_ty ptrT (zero_val ptrT) in
+      let: ("$ret0", "$ret1") := map.get (![mapT uint64T ptrT] (struct.field_ref Client "pending" (![ptrT] "cl"))) (![uint64T] "seqno") in
+      let: "$r0" := "$ret0" in
+      let: "$r1" := "$ret1" in
+      do:  ("cb" <-[ptrT] "$r0");;;
+      do:  ("ok" <-[boolT] "$r1");;;
+      (if: ![boolT] "ok"
+      then
+        do:  (MapDelete (![mapT uint64T ptrT] (struct.field_ref Client "pending" (![ptrT] "cl"))) (![uint64T] "seqno"));;;
+        let: "$r0" := ![sliceT byteT] "reply" in
+        do:  ((![ptrT] (struct.field_ref Callback "reply" (![ptrT] "cb"))) <-[sliceT byteT] "$r0");;;
+        let: "$r0" := callbackStateDone in
+        do:  ((![ptrT] (struct.field_ref Callback "state" (![ptrT] "cb"))) <-[uint64T] "$r0");;;
+        do:  ((sync.Cond__Signal (![ptrT] (struct.field_ref Callback "cond" (![ptrT] "cb")))) #());;;
+        do:  #()
+      else do:  #());;;
+      do:  ((sync.Mutex__Unlock (![ptrT] (struct.field_ref Client "mu" (![ptrT] "cl")))) #());;;
+      continue: #();;;
+      do:  #());;;
+    do:  #()).
+
+Definition Client__mset_ptr : list (string * val) := [
+  ("Call", Client__Call);
+  ("CallComplete", Client__CallComplete);
+  ("CallStart", Client__CallStart);
+  ("replyThread", Client__replyThread)
+].
+
+(* go: urpc.go:120:6 *)
+Definition TryMakeClient : val :=
+  rec: "TryMakeClient" "host_name" :=
+    exception_do (let: "host_name" := ref_ty uint64T "host_name" in
+    let: "host" := ref_ty uint64T (zero_val uint64T) in
+    let: "$r0" := ![uint64T] "host_name" in
+    do:  ("host" <-[uint64T] "$r0");;;
+    let: "a" := ref_ty grove_ffi.ConnectRet (zero_val grove_ffi.ConnectRet) in
+    let: "$r0" := let: "$a0" := ![uint64T] "host" in
+    grove_ffi.Connect "$a0" in
+    do:  ("a" <-[grove_ffi.ConnectRet] "$r0");;;
+    let: "nilClient" := ref_ty ptrT (zero_val ptrT) in
+    (if: ![boolT] (struct.field_ref grove_ffi.ConnectRet "Err" "a")
+    then
+      return: (#1, ![ptrT] "nilClient");;;
+      do:  #()
+    else do:  #());;;
+    let: "cl" := ref_ty ptrT (zero_val ptrT) in
+    let: "$r0" := ref_ty Client (struct.make Client [{
+      "conn" ::= ![grove_ffi.Connection] (struct.field_ref grove_ffi.ConnectRet "Connection" "a");
+      "mu" ::= ref_ty sync.Mutex (zero_val sync.Mutex);
+      "seq" ::= #1;
+      "pending" ::= map.make uint64T ptrT #()
+    }]) in
+    do:  ("cl" <-[ptrT] "$r0");;;
+    let: "$go" := (λ: <>,
+      do:  ((Client__replyThread (![ptrT] "cl")) #());;;
+      do:  #()
+      ) in
+    do:  (Fork ("$go" #()));;;
+    return: (#0, ![ptrT] "cl");;;
+    do:  #()).
+
+(* go: urpc.go:140:6 *)
+Definition MakeClient : val :=
+  rec: "MakeClient" "host_name" :=
+    exception_do (let: "host_name" := ref_ty uint64T "host_name" in
+    let: "cl" := ref_ty ptrT (zero_val ptrT) in
+    let: "err" := ref_ty uint64T (zero_val uint64T) in
+    let: ("$ret0", "$ret1") := let: "$a0" := ![uint64T] "host_name" in
+    TryMakeClient "$a0" in
+    let: "$r0" := "$ret0" in
+    let: "$r1" := "$ret1" in
+    do:  ("err" <-[uint64T] "$r0");;;
+    do:  ("cl" <-[ptrT] "$r1");;;
+    (if: (![uint64T] "err") ≠ #0
+    then
+      do:  (let: "$a0" := #(str "Unable to connect to %s") in
+      let: "$a1" := (let: "$sl0" := interface.make string__mset (let: "$a0" := ![uint64T] "host_name" in
+      grove_ffi.AddressToStr "$a0") in
+      slice.literal ["$sl0"]) in
+      log.Printf "$a0" "$a1");;;
+      do:  #()
+    else do:  #());;;
+    do:  (let: "$a0" := (![uint64T] "err") = #0 in
+    machine.Assume "$a0");;;
+    return: (![ptrT] "cl");;;
+    do:  #()).
+
+Definition Error : go_type := uint64T.
