new/code/github_com/mit_pdos/gokv/vrsm/paxos.v
@@ -11,8 +11,6 @@ From New.code Require sync.
 
 From New Require Import grove_prelude.
 
-(* internalclerk.go *)
-
 Definition RPC_APPLY_AS_FOLLOWER : expr := #0.
 
 Definition RPC_ENTER_NEW_EPOCH : expr := #1.
@@ -23,119 +21,49 @@ Definition singleClerk : go_type := structT [
   "cl" :: ptrT
 ].
 
-Definition MakeSingleClerk : val :=
-  rec: "MakeSingleClerk" "addr" :=
-    exception_do (let: "addr" := ref_ty uint64T "addr" in
-    let: "ck" := ref_ty ptrT (zero_val ptrT) in
-    let: "$a0" := ref_ty singleClerk (struct.make singleClerk [{
-      "cl" ::= reconnectclient.MakeReconnectingClient (![uint64T] "addr")
-    }]) in
-    do:  "ck" <-[ptrT] "$a0";;;
-    return: (![ptrT] "ck");;;
-    do:  #()).
+Definition singleClerk__mset : list (string * val) := [
+].
 
-(* Error from marshal.go *)
+(* go: internalclerk.go:51:23 *)
+Definition singleClerk__TryBecomeLeader : val :=
+  rec: "singleClerk__TryBecomeLeader" "s" <> :=
+    exception_do (let: "s" := ref_ty ptrT "s" in
+    let: "reply" := ref_ty ptrT (zero_val ptrT) in
+    let: "$r0" := ref_ty (sliceT byteT) (zero_val (sliceT byteT)) in
+    do:  ("reply" <-[ptrT] "$r0");;;
+    do:  (let: "$a0" := RPC_BECOME_LEADER in
+    let: "$a1" := slice.make2 byteT #0 in
+    let: "$a2" := ![ptrT] "reply" in
+    let: "$a3" := #500 in
+    (reconnectclient.ReconnectingClient__Call (![ptrT] (struct.field_ref singleClerk "cl" (![ptrT] "s")))) "$a0" "$a1" "$a2" "$a3");;;
+    do:  #()).
 
 Definition Error : go_type := uint64T.
-
-Definition enterNewEpochReply : go_type := structT [
-  "err" :: Error;
-  "acceptedEpoch" :: uint64T;
-  "nextIndex" :: uint64T;
-  "state" :: sliceT byteT
-].
-
-Definition ENone : expr := #0.
-
-Definition EEpochStale : expr := #1.
-
-Definition EOutOfOrder : expr := #2.
-
-Definition ETimeout : expr := #3.
-
-Definition ENotLeader : expr := #4.
-
-Definition decodeEnterNewEpochReply : val :=
-  rec: "decodeEnterNewEpochReply" "enc" :=
-    exception_do (let: "enc" := ref_ty (sliceT byteT) "enc" in
-    let: "o" := ref_ty ptrT (zero_val ptrT) in
-    let: "$a0" := ref_ty enterNewEpochReply (struct.make enterNewEpochReply [{
-    }]) in
-    do:  "o" <-[ptrT] "$a0";;;
-    let: "err" := ref_ty uint64T (zero_val uint64T) in
-    let: ("$a0", "$a1") := marshal.ReadInt (![sliceT byteT] "enc") in
-    do:  "enc" <-[sliceT byteT] "$a1";;;
-    do:  "err" <-[uint64T] "$a0";;;
-    let: "$a0" := ![uint64T] "err" in
-    do:  (struct.field_ref enterNewEpochReply "err" (![ptrT] "o")) <-[Error] "$a0";;;
-    let: ("$a0", "$a1") := marshal.ReadInt (![sliceT byteT] "enc") in
-    do:  "enc" <-[sliceT byteT] "$a1";;;
-    do:  (struct.field_ref enterNewEpochReply "acceptedEpoch" (![ptrT] "o")) <-[uint64T] "$a0";;;
-    let: ("$a0", "$a1") := marshal.ReadInt (![sliceT byteT] "enc") in
-    do:  "enc" <-[sliceT byteT] "$a1";;;
-    do:  (struct.field_ref enterNewEpochReply "nextIndex" (![ptrT] "o")) <-[uint64T] "$a0";;;
-    let: "$a0" := ![sliceT byteT] "enc" in
-    do:  (struct.field_ref enterNewEpochReply "state" (![ptrT] "o")) <-[sliceT byteT] "$a0";;;
-    return: (![ptrT] "o");;;
-    do:  #()).
-
-Definition enterNewEpochArgs : go_type := structT [
-  "epoch" :: uint64T
-].
-
-Definition encodeEnterNewEpochArgs : val :=
-  rec: "encodeEnterNewEpochArgs" "o" :=
-    exception_do (let: "o" := ref_ty ptrT "o" in
-    let: "enc" := ref_ty (sliceT byteT) (zero_val (sliceT byteT)) in
-    let: "$a0" := slice.make3 byteT #0 #8 in
-    do:  "enc" <-[sliceT byteT] "$a0";;;
-    let: "$a0" := marshal.WriteInt (![sliceT byteT] "enc") (![uint64T] (struct.field_ref enterNewEpochArgs "epoch" (![ptrT] "o"))) in
-    do:  "enc" <-[sliceT byteT] "$a0";;;
-    return: (![sliceT byteT] "enc");;;
-    do:  #()).
-
-Definition singleClerk__enterNewEpoch : val :=
-  rec: "singleClerk__enterNewEpoch" "s" "args" :=
-    exception_do (let: "s" := ref_ty ptrT "s" in
-    let: "args" := ref_ty ptrT "args" in
-    let: "raw_args" := ref_ty (sliceT byteT) (zero_val (sliceT byteT)) in
-    let: "$a0" := encodeEnterNewEpochArgs (![ptrT] "args") in
-    do:  "raw_args" <-[sliceT byteT] "$a0";;;
-    let: "raw_reply" := ref_ty ptrT (zero_val ptrT) in
-    let: "$a0" := ref_ty (sliceT byteT) (zero_val (sliceT byteT)) in
-    do:  "raw_reply" <-[ptrT] "$a0";;;
-    let: "err" := ref_ty uint64T (zero_val uint64T) in
-    let: "$a0" := (reconnectclient.ReconnectingClient__Call (![ptrT] (struct.field_ref singleClerk "cl" (![ptrT] "s")))) RPC_ENTER_NEW_EPOCH (![sliceT byteT] "raw_args") (![ptrT] "raw_reply") #500 in
-    do:  "err" <-[uint64T] "$a0";;;
-    (if: (![uint64T] "err") = #0
-    then
-      return: (decodeEnterNewEpochReply (![sliceT byteT] (![ptrT] "raw_reply")));;;
-      do:  #()
-    else
-      return: (ref_ty enterNewEpochReply (struct.make enterNewEpochReply [{
-         "err" ::= ETimeout
-       }]));;;
-      do:  #());;;
-    do:  #()).
 
 Definition applyAsFollowerReply : go_type := structT [
   "err" :: Error
 ].
 
+Definition ETimeout : expr := #3.
+
+(* go: marshal.go:41:6 *)
 Definition decodeApplyAsFollowerReply : val :=
   rec: "decodeApplyAsFollowerReply" "s" :=
     exception_do (let: "s" := ref_ty (sliceT byteT) "s" in
     let: "o" := ref_ty ptrT (zero_val ptrT) in
-    let: "$a0" := ref_ty applyAsFollowerReply (struct.make applyAsFollowerReply [{
+    let: "$r0" := ref_ty applyAsFollowerReply (struct.make applyAsFollowerReply [{
     }]) in
-    do:  "o" <-[ptrT] "$a0";;;
+    do:  ("o" <-[ptrT] "$r0");;;
     let: <> := ref_ty (sliceT byteT) (zero_val (sliceT byteT)) in
     let: "err" := ref_ty uint64T (zero_val uint64T) in
-    let: ("$a0", "$a1") := marshal.ReadInt (![sliceT byteT] "s") in
-    do:  "$a1";;;
-    do:  "err" <-[uint64T] "$a0";;;
-    let: "$a0" := ![uint64T] "err" in
-    do:  (struct.field_ref applyAsFollowerReply "err" (![ptrT] "o")) <-[Error] "$a0";;;
+    let: ("$ret0", "$ret1") := let: "$a0" := ![sliceT byteT] "s" in
+    marshal.ReadInt "$a0" in
+    let: "$r0" := "$ret0" in
+    let: "$r1" := "$ret1" in
+    do:  ("err" <-[uint64T] "$r0");;;
+    do:  "$r1";;;
+    let: "$r0" := ![uint64T] "err" in
+    do:  ((struct.field_ref applyAsFollowerReply "err" (![ptrT] "o")) <-[Error] "$r0");;;
     return: (![ptrT] "o");;;
     do:  #()).
 
@@ -145,37 +73,51 @@ Definition applyAsFollowerArgs : go_type := structT [
   "state" :: sliceT byteT
 ].
 
+(* go: marshal.go:21:6 *)
 Definition encodeApplyAsFollowerArgs : val :=
   rec: "encodeApplyAsFollowerArgs" "o" :=
     exception_do (let: "o" := ref_ty ptrT "o" in
     let: "enc" := ref_ty (sliceT byteT) (zero_val (sliceT byteT)) in
-    let: "$a0" := slice.make3 byteT #0 ((#8 + #8) + (slice.len (![sliceT byteT] (struct.field_ref applyAsFollowerArgs "state" (![ptrT] "o"))))) in
-    do:  "enc" <-[sliceT byteT] "$a0";;;
-    let: "$a0" := marshal.WriteInt (![sliceT byteT] "enc") (![uint64T] (struct.field_ref applyAsFollowerArgs "epoch" (![ptrT] "o"))) in
-    do:  "enc" <-[sliceT byteT] "$a0";;;
-    let: "$a0" := marshal.WriteInt (![sliceT byteT] "enc") (![uint64T] (struct.field_ref applyAsFollowerArgs "nextIndex" (![ptrT] "o"))) in
-    do:  "enc" <-[sliceT byteT] "$a0";;;
-    let: "$a0" := marshal.WriteBytes (![sliceT byteT] "enc") (![sliceT byteT] (struct.field_ref applyAsFollowerArgs "state" (![ptrT] "o"))) in
-    do:  "enc" <-[sliceT byteT] "$a0";;;
+    let: "$r0" := slice.make3 byteT #0 ((#8 + #8) + (slice.len (![sliceT byteT] (struct.field_ref applyAsFollowerArgs "state" (![ptrT] "o"))))) in
+    do:  ("enc" <-[sliceT byteT] "$r0");;;
+    let: "$r0" := let: "$a0" := ![sliceT byteT] "enc" in
+    let: "$a1" := ![uint64T] (struct.field_ref applyAsFollowerArgs "epoch" (![ptrT] "o")) in
+    marshal.WriteInt "$a0" "$a1" in
+    do:  ("enc" <-[sliceT byteT] "$r0");;;
+    let: "$r0" := let: "$a0" := ![sliceT byteT] "enc" in
+    let: "$a1" := ![uint64T] (struct.field_ref applyAsFollowerArgs "nextIndex" (![ptrT] "o")) in
+    marshal.WriteInt "$a0" "$a1" in
+    do:  ("enc" <-[sliceT byteT] "$r0");;;
+    let: "$r0" := let: "$a0" := ![sliceT byteT] "enc" in
+    let: "$a1" := ![sliceT byteT] (struct.field_ref applyAsFollowerArgs "state" (![ptrT] "o")) in
+    marshal.WriteBytes "$a0" "$a1" in
+    do:  ("enc" <-[sliceT byteT] "$r0");;;
     return: (![sliceT byteT] "enc");;;
     do:  #()).
 
+(* go: internalclerk.go:40:23 *)
 Definition singleClerk__applyAsFollower : val :=
   rec: "singleClerk__applyAsFollower" "s" "args" :=
     exception_do (let: "s" := ref_ty ptrT "s" in
     let: "args" := ref_ty ptrT "args" in
     let: "raw_args" := ref_ty (sliceT byteT) (zero_val (sliceT byteT)) in
-    let: "$a0" := encodeApplyAsFollowerArgs (![ptrT] "args") in
-    do:  "raw_args" <-[sliceT byteT] "$a0";;;
+    let: "$r0" := let: "$a0" := ![ptrT] "args" in
+    encodeApplyAsFollowerArgs "$a0" in
+    do:  ("raw_args" <-[sliceT byteT] "$r0");;;
     let: "raw_reply" := ref_ty ptrT (zero_val ptrT) in
-    let: "$a0" := ref_ty (sliceT byteT) (zero_val (sliceT byteT)) in
-    do:  "raw_reply" <-[ptrT] "$a0";;;
+    let: "$r0" := ref_ty (sliceT byteT) (zero_val (sliceT byteT)) in
+    do:  ("raw_reply" <-[ptrT] "$r0");;;
     let: "err" := ref_ty uint64T (zero_val uint64T) in
-    let: "$a0" := (reconnectclient.ReconnectingClient__Call (![ptrT] (struct.field_ref singleClerk "cl" (![ptrT] "s")))) RPC_APPLY_AS_FOLLOWER (![sliceT byteT] "raw_args") (![ptrT] "raw_reply") #500 in
-    do:  "err" <-[uint64T] "$a0";;;
+    let: "$r0" := let: "$a0" := RPC_APPLY_AS_FOLLOWER in
+    let: "$a1" := ![sliceT byteT] "raw_args" in
+    let: "$a2" := ![ptrT] "raw_reply" in
+    let: "$a3" := #500 in
+    (reconnectclient.ReconnectingClient__Call (![ptrT] (struct.field_ref singleClerk "cl" (![ptrT] "s")))) "$a0" "$a1" "$a2" "$a3" in
+    do:  ("err" <-[uint64T] "$r0");;;
     (if: (![uint64T] "err") = #0
     then
-      return: (decodeApplyAsFollowerReply (![sliceT byteT] (![ptrT] "raw_reply")));;;
+      return: (let: "$a0" := ![sliceT byteT] (![ptrT] "raw_reply") in
+       decodeApplyAsFollowerReply "$a0");;;
       do:  #()
     else
       return: (ref_ty applyAsFollowerReply (struct.make applyAsFollowerReply [{
@@ -184,71 +126,230 @@ Definition singleClerk__applyAsFollower : val :=
       do:  #());;;
     do:  #()).
 
-Definition singleClerk__TryBecomeLeader : val :=
-  rec: "singleClerk__TryBecomeLeader" "s" <> :=
-    exception_do (let: "s" := ref_ty ptrT "s" in
-    let: "reply" := ref_ty ptrT (zero_val ptrT) in
-    let: "$a0" := ref_ty (sliceT byteT) (zero_val (sliceT byteT)) in
-    do:  "reply" <-[ptrT] "$a0";;;
-    do:  (reconnectclient.ReconnectingClient__Call (![ptrT] (struct.field_ref singleClerk "cl" (![ptrT] "s")))) RPC_BECOME_LEADER (slice.make2 byteT #0) (![ptrT] "reply") #500;;;
+Definition enterNewEpochReply : go_type := structT [
+  "err" :: Error;
+  "acceptedEpoch" :: uint64T;
+  "nextIndex" :: uint64T;
+  "state" :: sliceT byteT
+].
+
+(* go: marshal.go:77:6 *)
+Definition decodeEnterNewEpochReply : val :=
+  rec: "decodeEnterNewEpochReply" "enc" :=
+    exception_do (let: "enc" := ref_ty (sliceT byteT) "enc" in
+    let: "o" := ref_ty ptrT (zero_val ptrT) in
+    let: "$r0" := ref_ty enterNewEpochReply (struct.make enterNewEpochReply [{
+    }]) in
+    do:  ("o" <-[ptrT] "$r0");;;
+    let: "err" := ref_ty uint64T (zero_val uint64T) in
+    let: ("$ret0", "$ret1") := let: "$a0" := ![sliceT byteT] "enc" in
+    marshal.ReadInt "$a0" in
+    let: "$r0" := "$ret0" in
+    let: "$r1" := "$ret1" in
+    do:  ("err" <-[uint64T] "$r0");;;
+    do:  ("enc" <-[sliceT byteT] "$r1");;;
+    let: "$r0" := ![uint64T] "err" in
+    do:  ((struct.field_ref enterNewEpochReply "err" (![ptrT] "o")) <-[Error] "$r0");;;
+    let: ("$ret0", "$ret1") := let: "$a0" := ![sliceT byteT] "enc" in
+    marshal.ReadInt "$a0" in
+    let: "$r0" := "$ret0" in
+    let: "$r1" := "$ret1" in
+    do:  ((struct.field_ref enterNewEpochReply "acceptedEpoch" (![ptrT] "o")) <-[uint64T] "$r0");;;
+    do:  ("enc" <-[sliceT byteT] "$r1");;;
+    let: ("$ret0", "$ret1") := let: "$a0" := ![sliceT byteT] "enc" in
+    marshal.ReadInt "$a0" in
+    let: "$r0" := "$ret0" in
+    let: "$r1" := "$ret1" in
+    do:  ((struct.field_ref enterNewEpochReply "nextIndex" (![ptrT] "o")) <-[uint64T] "$r0");;;
+    do:  ("enc" <-[sliceT byteT] "$r1");;;
+    let: "$r0" := ![sliceT byteT] "enc" in
+    do:  ((struct.field_ref enterNewEpochReply "state" (![ptrT] "o")) <-[sliceT byteT] "$r0");;;
+    return: (![ptrT] "o");;;
     do:  #()).
 
-(* marshal.go *)
+Definition enterNewEpochArgs : go_type := structT [
+  "epoch" :: uint64T
+].
 
+(* go: marshal.go:58:6 *)
+Definition encodeEnterNewEpochArgs : val :=
+  rec: "encodeEnterNewEpochArgs" "o" :=
+    exception_do (let: "o" := ref_ty ptrT "o" in
+    let: "enc" := ref_ty (sliceT byteT) (zero_val (sliceT byteT)) in
+    let: "$r0" := slice.make3 byteT #0 #8 in
+    do:  ("enc" <-[sliceT byteT] "$r0");;;
+    let: "$r0" := let: "$a0" := ![sliceT byteT] "enc" in
+    let: "$a1" := ![uint64T] (struct.field_ref enterNewEpochArgs "epoch" (![ptrT] "o")) in
+    marshal.WriteInt "$a0" "$a1" in
+    do:  ("enc" <-[sliceT byteT] "$r0");;;
+    return: (![sliceT byteT] "enc");;;
+    do:  #()).
+
+(* go: internalclerk.go:28:23 *)
+Definition singleClerk__enterNewEpoch : val :=
+  rec: "singleClerk__enterNewEpoch" "s" "args" :=
+    exception_do (let: "s" := ref_ty ptrT "s" in
+    let: "args" := ref_ty ptrT "args" in
+    let: "raw_args" := ref_ty (sliceT byteT) (zero_val (sliceT byteT)) in
+    let: "$r0" := let: "$a0" := ![ptrT] "args" in
+    encodeEnterNewEpochArgs "$a0" in
+    do:  ("raw_args" <-[sliceT byteT] "$r0");;;
+    let: "raw_reply" := ref_ty ptrT (zero_val ptrT) in
+    let: "$r0" := ref_ty (sliceT byteT) (zero_val (sliceT byteT)) in
+    do:  ("raw_reply" <-[ptrT] "$r0");;;
+    let: "err" := ref_ty uint64T (zero_val uint64T) in
+    let: "$r0" := let: "$a0" := RPC_ENTER_NEW_EPOCH in
+    let: "$a1" := ![sliceT byteT] "raw_args" in
+    let: "$a2" := ![ptrT] "raw_reply" in
+    let: "$a3" := #500 in
+    (reconnectclient.ReconnectingClient__Call (![ptrT] (struct.field_ref singleClerk "cl" (![ptrT] "s")))) "$a0" "$a1" "$a2" "$a3" in
+    do:  ("err" <-[uint64T] "$r0");;;
+    (if: (![uint64T] "err") = #0
+    then
+      return: (let: "$a0" := ![sliceT byteT] (![ptrT] "raw_reply") in
+       decodeEnterNewEpochReply "$a0");;;
+      do:  #()
+    else
+      return: (ref_ty enterNewEpochReply (struct.make enterNewEpochReply [{
+         "err" ::= ETimeout
+       }]));;;
+      do:  #());;;
+    do:  #()).
+
+Definition singleClerk__mset_ptr : list (string * val) := [
+  ("TryBecomeLeader", singleClerk__TryBecomeLeader);
+  ("applyAsFollower", singleClerk__applyAsFollower);
+  ("enterNewEpoch", singleClerk__enterNewEpoch)
+].
+
+(* go: internalclerk.go:19:6 *)
+Definition MakeSingleClerk : val :=
+  rec: "MakeSingleClerk" "addr" :=
+    exception_do (let: "addr" := ref_ty uint64T "addr" in
+    let: "ck" := ref_ty ptrT (zero_val ptrT) in
+    let: "$r0" := ref_ty singleClerk (struct.make singleClerk [{
+      "cl" ::= let: "$a0" := ![uint64T] "addr" in
+      reconnectclient.MakeReconnectingClient "$a0"
+    }]) in
+    do:  ("ck" <-[ptrT] "$r0");;;
+    return: (![ptrT] "ck");;;
+    do:  #()).
+
+Definition Error__mset : list (string * val) := [
+].
+
+Definition Error__mset_ptr : list (string * val) := [
+].
+
+Definition ENone : expr := #0.
+
+Definition EEpochStale : expr := #1.
+
+Definition EOutOfOrder : expr := #2.
+
+Definition ENotLeader : expr := #4.
+
+Definition applyAsFollowerArgs__mset : list (string * val) := [
+].
+
+Definition applyAsFollowerArgs__mset_ptr : list (string * val) := [
+].
+
+(* go: marshal.go:29:6 *)
 Definition decodeApplyAsFollowerArgs : val :=
   rec: "decodeApplyAsFollowerArgs" "enc" :=
     exception_do (let: "enc" := ref_ty (sliceT byteT) "enc" in
     let: "o" := ref_ty ptrT (zero_val ptrT) in
-    let: "$a0" := ref_ty applyAsFollowerArgs (zero_val applyAsFollowerArgs) in
-    do:  "o" <-[ptrT] "$a0";;;
-    let: ("$a0", "$a1") := marshal.ReadInt (![sliceT byteT] "enc") in
-    do:  "enc" <-[sliceT byteT] "$a1";;;
-    do:  (struct.field_ref applyAsFollowerArgs "epoch" (![ptrT] "o")) <-[uint64T] "$a0";;;
-    let: ("$a0", "$a1") := marshal.ReadInt (![sliceT byteT] "enc") in
-    do:  "enc" <-[sliceT byteT] "$a1";;;
-    do:  (struct.field_ref applyAsFollowerArgs "nextIndex" (![ptrT] "o")) <-[uint64T] "$a0";;;
-    let: "$a0" := ![sliceT byteT] "enc" in
-    do:  (struct.field_ref applyAsFollowerArgs "state" (![ptrT] "o")) <-[sliceT byteT] "$a0";;;
+    let: "$r0" := ref_ty applyAsFollowerArgs (zero_val applyAsFollowerArgs) in
+    do:  ("o" <-[ptrT] "$r0");;;
+    let: ("$ret0", "$ret1") := let: "$a0" := ![sliceT byteT] "enc" in
+    marshal.ReadInt "$a0" in
+    let: "$r0" := "$ret0" in
+    let: "$r1" := "$ret1" in
+    do:  ((struct.field_ref applyAsFollowerArgs "epoch" (![ptrT] "o")) <-[uint64T] "$r0");;;
+    do:  ("enc" <-[sliceT byteT] "$r1");;;
+    let: ("$ret0", "$ret1") := let: "$a0" := ![sliceT byteT] "enc" in
+    marshal.ReadInt "$a0" in
+    let: "$r0" := "$ret0" in
+    let: "$r1" := "$ret1" in
+    do:  ((struct.field_ref applyAsFollowerArgs "nextIndex" (![ptrT] "o")) <-[uint64T] "$r0");;;
+    do:  ("enc" <-[sliceT byteT] "$r1");;;
+    let: "$r0" := ![sliceT byteT] "enc" in
+    do:  ((struct.field_ref applyAsFollowerArgs "state" (![ptrT] "o")) <-[sliceT byteT] "$r0");;;
     return: (![ptrT] "o");;;
     do:  #()).
 
+Definition applyAsFollowerReply__mset : list (string * val) := [
+].
+
+Definition applyAsFollowerReply__mset_ptr : list (string * val) := [
+].
+
+(* go: marshal.go:48:6 *)
 Definition encodeApplyAsFollowerReply : val :=
   rec: "encodeApplyAsFollowerReply" "o" :=
     exception_do (let: "o" := ref_ty ptrT "o" in
     let: "enc" := ref_ty (sliceT byteT) (zero_val (sliceT byteT)) in
-    let: "$a0" := slice.make3 byteT #0 #8 in
-    do:  "enc" <-[sliceT byteT] "$a0";;;
-    let: "$a0" := marshal.WriteInt (![sliceT byteT] "enc") (![Error] (struct.field_ref applyAsFollowerReply "err" (![ptrT] "o"))) in
-    do:  "enc" <-[sliceT byteT] "$a0";;;
+    let: "$r0" := slice.make3 byteT #0 #8 in
+    do:  ("enc" <-[sliceT byteT] "$r0");;;
+    let: "$r0" := let: "$a0" := ![sliceT byteT] "enc" in
+    let: "$a1" := ![Error] (struct.field_ref applyAsFollowerReply "err" (![ptrT] "o")) in
+    marshal.WriteInt "$a0" "$a1" in
+    do:  ("enc" <-[sliceT byteT] "$r0");;;
     return: (![sliceT byteT] "enc");;;
     do:  #()).
 
+Definition enterNewEpochArgs__mset : list (string * val) := [
+].
+
+Definition enterNewEpochArgs__mset_ptr : list (string * val) := [
+].
+
+(* go: marshal.go:64:6 *)
 Definition decodeEnterNewEpochArgs : val :=
   rec: "decodeEnterNewEpochArgs" "s" :=
     exception_do (let: "s" := ref_ty (sliceT byteT) "s" in
     let: "o" := ref_ty ptrT (zero_val ptrT) in
-    let: "$a0" := ref_ty enterNewEpochArgs (zero_val enterNewEpochArgs) in
-    do:  "o" <-[ptrT] "$a0";;;
-    let: ("$a0", "$a1") := marshal.ReadInt (![sliceT byteT] "s") in
-    do:  "$a1";;;
-    do:  (struct.field_ref enterNewEpochArgs "epoch" (![ptrT] "o")) <-[uint64T] "$a0";;;
+    let: "$r0" := ref_ty enterNewEpochArgs (zero_val enterNewEpochArgs) in
+    do:  ("o" <-[ptrT] "$r0");;;
+    let: ("$ret0", "$ret1") := let: "$a0" := ![sliceT byteT] "s" in
+    marshal.ReadInt "$a0" in
+    let: "$r0" := "$ret0" in
+    let: "$r1" := "$ret1" in
+    do:  ((struct.field_ref enterNewEpochArgs "epoch" (![ptrT] "o")) <-[uint64T] "$r0");;;
+    do:  "$r1";;;
     return: (![ptrT] "o");;;
     do:  #()).
 
+Definition enterNewEpochReply__mset : list (string * val) := [
+].
+
+Definition enterNewEpochReply__mset_ptr : list (string * val) := [
+].
+
+(* go: marshal.go:89:6 *)
 Definition encodeEnterNewEpochReply : val :=
   rec: "encodeEnterNewEpochReply" "o" :=
     exception_do (let: "o" := ref_ty ptrT "o" in
     let: "enc" := ref_ty (sliceT byteT) (zero_val (sliceT byteT)) in
-    let: "$a0" := slice.make3 byteT #0 (((#8 + #8) + #8) + (slice.len (![sliceT byteT] (struct.field_ref enterNewEpochReply "state" (![ptrT] "o"))))) in
-    do:  "enc" <-[sliceT byteT] "$a0";;;
-    let: "$a0" := marshal.WriteInt (![sliceT byteT] "enc") (![Error] (struct.field_ref enterNewEpochReply "err" (![ptrT] "o"))) in
-    do:  "enc" <-[sliceT byteT] "$a0";;;
-    let: "$a0" := marshal.WriteInt (![sliceT byteT] "enc") (![uint64T] (struct.field_ref enterNewEpochReply "acceptedEpoch" (![ptrT] "o"))) in
-    do:  "enc" <-[sliceT byteT] "$a0";;;
-    let: "$a0" := marshal.WriteInt (![sliceT byteT] "enc") (![uint64T] (struct.field_ref enterNewEpochReply "nextIndex" (![ptrT] "o"))) in
-    do:  "enc" <-[sliceT byteT] "$a0";;;
-    let: "$a0" := marshal.WriteBytes (![sliceT byteT] "enc") (![sliceT byteT] (struct.field_ref enterNewEpochReply "state" (![ptrT] "o"))) in
-    do:  "enc" <-[sliceT byteT] "$a0";;;
+    let: "$r0" := slice.make3 byteT #0 (((#8 + #8) + #8) + (slice.len (![sliceT byteT] (struct.field_ref enterNewEpochReply "state" (![ptrT] "o"))))) in
+    do:  ("enc" <-[sliceT byteT] "$r0");;;
+    let: "$r0" := let: "$a0" := ![sliceT byteT] "enc" in
+    let: "$a1" := ![Error] (struct.field_ref enterNewEpochReply "err" (![ptrT] "o")) in
+    marshal.WriteInt "$a0" "$a1" in
+    do:  ("enc" <-[sliceT byteT] "$r0");;;
+    let: "$r0" := let: "$a0" := ![sliceT byteT] "enc" in
+    let: "$a1" := ![uint64T] (struct.field_ref enterNewEpochReply "acceptedEpoch" (![ptrT] "o")) in
+    marshal.WriteInt "$a0" "$a1" in
+    do:  ("enc" <-[sliceT byteT] "$r0");;;
+    let: "$r0" := let: "$a0" := ![sliceT byteT] "enc" in
+    let: "$a1" := ![uint64T] (struct.field_ref enterNewEpochReply "nextIndex" (![ptrT] "o")) in
+    marshal.WriteInt "$a0" "$a1" in
+    do:  ("enc" <-[sliceT byteT] "$r0");;;
+    let: "$r0" := let: "$a0" := ![sliceT byteT] "enc" in
+    let: "$a1" := ![sliceT byteT] (struct.field_ref enterNewEpochReply "state" (![ptrT] "o")) in
+    marshal.WriteBytes "$a0" "$a1" in
+    do:  ("enc" <-[sliceT byteT] "$r0");;;
     return: (![sliceT byteT] "enc");;;
     do:  #()).
 
@@ -257,37 +358,53 @@ Definition applyReply : go_type := structT [
   "ret" :: sliceT byteT
 ].
 
+Definition applyReply__mset : list (string * val) := [
+].
+
+Definition applyReply__mset_ptr : list (string * val) := [
+].
+
+(* go: marshal.go:103:6 *)
 Definition encodeApplyReply : val :=
   rec: "encodeApplyReply" "o" :=
     exception_do (let: "o" := ref_ty ptrT "o" in
     let: "enc" := ref_ty (sliceT byteT) (zero_val (sliceT byteT)) in
-    let: "$a0" := slice.make3 byteT #0 (#8 + (slice.len (![sliceT byteT] (struct.field_ref applyReply "ret" (![ptrT] "o"))))) in
-    do:  "enc" <-[sliceT byteT] "$a0";;;
-    let: "$a0" := marshal.WriteInt (![sliceT byteT] "enc") (![Error] (struct.field_ref applyReply "err" (![ptrT] "o"))) in
-    do:  "enc" <-[sliceT byteT] "$a0";;;
-    let: "$a0" := marshal.WriteBytes (![sliceT byteT] "enc") (![sliceT byteT] (struct.field_ref applyReply "ret" (![ptrT] "o"))) in
-    do:  "enc" <-[sliceT byteT] "$a0";;;
+    let: "$r0" := slice.make3 byteT #0 (#8 + (slice.len (![sliceT byteT] (struct.field_ref applyReply "ret" (![ptrT] "o"))))) in
+    do:  ("enc" <-[sliceT byteT] "$r0");;;
+    let: "$r0" := let: "$a0" := ![sliceT byteT] "enc" in
+    let: "$a1" := ![Error] (struct.field_ref applyReply "err" (![ptrT] "o")) in
+    marshal.WriteInt "$a0" "$a1" in
+    do:  ("enc" <-[sliceT byteT] "$r0");;;
+    let: "$r0" := let: "$a0" := ![sliceT byteT] "enc" in
+    let: "$a1" := ![sliceT byteT] (struct.field_ref applyReply "ret" (![ptrT] "o")) in
+    marshal.WriteBytes "$a0" "$a1" in
+    do:  ("enc" <-[sliceT byteT] "$r0");;;
     return: (![sliceT byteT] "enc");;;
     do:  #()).
 
+(* go: marshal.go:110:6 *)
 Definition decodeApplyReply : val :=
   rec: "decodeApplyReply" "enc" :=
     exception_do (let: "enc" := ref_ty (sliceT byteT) "enc" in
     let: "o" := ref_ty ptrT (zero_val ptrT) in
-    let: "$a0" := ref_ty applyReply (struct.make applyReply [{
+    let: "$r0" := ref_ty applyReply (struct.make applyReply [{
     }]) in
-    do:  "o" <-[ptrT] "$a0";;;
+    do:  ("o" <-[ptrT] "$r0");;;
     let: "err" := ref_ty uint64T (zero_val uint64T) in
-    let: ("$a0", "$a1") := marshal.ReadInt (![sliceT byteT] "enc") in
-    do:  "enc" <-[sliceT byteT] "$a1";;;
-    do:  "err" <-[uint64T] "$a0";;;
-    let: "$a0" := ![uint64T] "err" in
-    do:  (struct.field_ref applyReply "err" (![ptrT] "o")) <-[Error] "$a0";;;
-    let: "$a0" := ![sliceT byteT] "enc" in
-    do:  (struct.field_ref applyReply "ret" (![ptrT] "o")) <-[sliceT byteT] "$a0";;;
+    let: ("$ret0", "$ret1") := let: "$a0" := ![sliceT byteT] "enc" in
+    marshal.ReadInt "$a0" in
+    let: "$r0" := "$ret0" in
+    let: "$r1" := "$ret1" in
+    do:  ("err" <-[uint64T] "$r0");;;
+    do:  ("enc" <-[sliceT byteT] "$r1");;;
+    let: "$r0" := ![uint64T] "err" in
+    do:  ((struct.field_ref applyReply "err" (![ptrT] "o")) <-[Error] "$r0");;;
+    let: "$r0" := ![sliceT byteT] "enc" in
+    do:  ((struct.field_ref applyReply "ret" (![ptrT] "o")) <-[sliceT byteT] "$r0");;;
     return: (![ptrT] "o");;;
     do:  #()).
 
+(* go: marshal.go:120:6 *)
 Definition boolToU64 : val :=
   rec: "boolToU64" "b" :=
     exception_do (let: "b" := ref_ty boolT "b" in
@@ -300,8 +417,6 @@ Definition boolToU64 : val :=
       do:  #());;;
     do:  #()).
 
-(* paxosState from server.go *)
-
 Definition paxosState : go_type := structT [
   "epoch" :: uint64T;
   "acceptedEpoch" :: uint64T;
@@ -310,49 +425,78 @@ Definition paxosState : go_type := structT [
   "isLeader" :: boolT
 ].
 
+(* go: marshal.go:128:6 *)
 Definition encodePaxosState : val :=
   rec: "encodePaxosState" "ps" :=
     exception_do (let: "ps" := ref_ty ptrT "ps" in
     let: "e" := ref_ty (sliceT byteT) (slice.make2 byteT #0) in
-    let: "$a0" := marshal.WriteInt (![sliceT byteT] "e") (![uint64T] (struct.field_ref paxosState "epoch" (![ptrT] "ps"))) in
-    do:  "e" <-[sliceT byteT] "$a0";;;
-    let: "$a0" := marshal.WriteInt (![sliceT byteT] "e") (![uint64T] (struct.field_ref paxosState "acceptedEpoch" (![ptrT] "ps"))) in
-    do:  "e" <-[sliceT byteT] "$a0";;;
-    let: "$a0" := marshal.WriteInt (![sliceT byteT] "e") (![uint64T] (struct.field_ref paxosState "nextIndex" (![ptrT] "ps"))) in
-    do:  "e" <-[sliceT byteT] "$a0";;;
-    let: "$a0" := marshal.WriteInt (![sliceT byteT] "e") (boolToU64 (![boolT] (struct.field_ref paxosState "isLeader" (![ptrT] "ps")))) in
-    do:  "e" <-[sliceT byteT] "$a0";;;
-    let: "$a0" := marshal.WriteBytes (![sliceT byteT] "e") (![sliceT byteT] (struct.field_ref paxosState "state" (![ptrT] "ps"))) in
-    do:  "e" <-[sliceT byteT] "$a0";;;
+    let: "$r0" := let: "$a0" := ![sliceT byteT] "e" in
+    let: "$a1" := ![uint64T] (struct.field_ref paxosState "epoch" (![ptrT] "ps")) in
+    marshal.WriteInt "$a0" "$a1" in
+    do:  ("e" <-[sliceT byteT] "$r0");;;
+    let: "$r0" := let: "$a0" := ![sliceT byteT] "e" in
+    let: "$a1" := ![uint64T] (struct.field_ref paxosState "acceptedEpoch" (![ptrT] "ps")) in
+    marshal.WriteInt "$a0" "$a1" in
+    do:  ("e" <-[sliceT byteT] "$r0");;;
+    let: "$r0" := let: "$a0" := ![sliceT byteT] "e" in
+    let: "$a1" := ![uint64T] (struct.field_ref paxosState "nextIndex" (![ptrT] "ps")) in
+    marshal.WriteInt "$a0" "$a1" in
+    do:  ("e" <-[sliceT byteT] "$r0");;;
+    let: "$r0" := let: "$a0" := ![sliceT byteT] "e" in
+    let: "$a1" := let: "$a0" := ![boolT] (struct.field_ref paxosState "isLeader" (![ptrT] "ps")) in
+    boolToU64 "$a0" in
+    marshal.WriteInt "$a0" "$a1" in
+    do:  ("e" <-[sliceT byteT] "$r0");;;
+    let: "$r0" := let: "$a0" := ![sliceT byteT] "e" in
+    let: "$a1" := ![sliceT byteT] (struct.field_ref paxosState "state" (![ptrT] "ps")) in
+    marshal.WriteBytes "$a0" "$a1" in
+    do:  ("e" <-[sliceT byteT] "$r0");;;
     return: (![sliceT byteT] "e");;;
     do:  #()).
 
+(* go: marshal.go:138:6 *)
 Definition decodePaxosState : val :=
   rec: "decodePaxosState" "enc" :=
     exception_do (let: "enc" := ref_ty (sliceT byteT) "enc" in
     let: "e" := ref_ty (sliceT byteT) (![sliceT byteT] "enc") in
     let: "leaderInt" := ref_ty uint64T (zero_val uint64T) in
     let: "ps" := ref_ty ptrT (zero_val ptrT) in
-    let: "$a0" := ref_ty paxosState (zero_val paxosState) in
-    do:  "ps" <-[ptrT] "$a0";;;
-    let: ("$a0", "$a1") := marshal.ReadInt (![sliceT byteT] "e") in
-    do:  "e" <-[sliceT byteT] "$a1";;;
-    do:  (struct.field_ref paxosState "epoch" (![ptrT] "ps")) <-[uint64T] "$a0";;;
-    let: ("$a0", "$a1") := marshal.ReadInt (![sliceT byteT] "e") in
-    do:  "e" <-[sliceT byteT] "$a1";;;
-    do:  (struct.field_ref paxosState "acceptedEpoch" (![ptrT] "ps")) <-[uint64T] "$a0";;;
-    let: ("$a0", "$a1") := marshal.ReadInt (![sliceT byteT] "e") in
-    do:  "e" <-[sliceT byteT] "$a1";;;
-    do:  (struct.field_ref paxosState "nextIndex" (![ptrT] "ps")) <-[uint64T] "$a0";;;
-    let: ("$a0", "$a1") := marshal.ReadInt (![sliceT byteT] "e") in
-    do:  (struct.field_ref paxosState "state" (![ptrT] "ps")) <-[sliceT byteT] "$a1";;;
-    do:  "leaderInt" <-[uint64T] "$a0";;;
-    let: "$a0" := (![uint64T] "leaderInt") = #1 in
-    do:  (struct.field_ref paxosState "isLeader" (![ptrT] "ps")) <-[boolT] "$a0";;;
+    let: "$r0" := ref_ty paxosState (zero_val paxosState) in
+    do:  ("ps" <-[ptrT] "$r0");;;
+    let: ("$ret0", "$ret1") := let: "$a0" := ![sliceT byteT] "e" in
+    marshal.ReadInt "$a0" in
+    let: "$r0" := "$ret0" in
+    let: "$r1" := "$ret1" in
+    do:  ((struct.field_ref paxosState "epoch" (![ptrT] "ps")) <-[uint64T] "$r0");;;
+    do:  ("e" <-[sliceT byteT] "$r1");;;
+    let: ("$ret0", "$ret1") := let: "$a0" := ![sliceT byteT] "e" in
+    marshal.ReadInt "$a0" in
+    let: "$r0" := "$ret0" in
+    let: "$r1" := "$ret1" in
+    do:  ((struct.field_ref paxosState "acceptedEpoch" (![ptrT] "ps")) <-[uint64T] "$r0");;;
+    do:  ("e" <-[sliceT byteT] "$r1");;;
+    let: ("$ret0", "$ret1") := let: "$a0" := ![sliceT byteT] "e" in
+    marshal.ReadInt "$a0" in
+    let: "$r0" := "$ret0" in
+    let: "$r1" := "$ret1" in
+    do:  ((struct.field_ref paxosState "nextIndex" (![ptrT] "ps")) <-[uint64T] "$r0");;;
+    do:  ("e" <-[sliceT byteT] "$r1");;;
+    let: ("$ret0", "$ret1") := let: "$a0" := ![sliceT byteT] "e" in
+    marshal.ReadInt "$a0" in
+    let: "$r0" := "$ret0" in
+    let: "$r1" := "$ret1" in
+    do:  ("leaderInt" <-[uint64T] "$r0");;;
+    do:  ((struct.field_ref paxosState "state" (![ptrT] "ps")) <-[sliceT byteT] "$r1");;;
+    let: "$r0" := (![uint64T] "leaderInt") = #1 in
+    do:  ((struct.field_ref paxosState "isLeader" (![ptrT] "ps")) <-[boolT] "$r0");;;
     return: (![ptrT] "ps");;;
     do:  #()).
 
-(* server.go *)
+Definition paxosState__mset : list (string * val) := [
+].
+
+Definition paxosState__mset_ptr : list (string * val) := [
+].
 
 Definition Server : go_type := structT [
   "mu" :: ptrT;
@@ -361,163 +505,209 @@ Definition Server : go_type := structT [
   "clerks" :: sliceT ptrT
 ].
 
+Definition Server__mset : list (string * val) := [
+].
+
+(* go: server.go:165:18 *)
+Definition Server__TryAcquire : val :=
+  rec: "Server__TryAcquire" "s" <> :=
+    exception_do (let: "s" := ref_ty ptrT "s" in
+    let: "retErr" := ref_ty Error (zero_val Error) in
+    do:  ((sync.Mutex__Lock (![ptrT] (struct.field_ref Server "mu" (![ptrT] "s")))) #());;;
+    (if: (~ (![boolT] (struct.field_ref paxosState "isLeader" (![ptrT] (struct.field_ref Server "ps" (![ptrT] "s"))))))
+    then
+      do:  ((sync.Mutex__Unlock (![ptrT] (struct.field_ref Server "mu" (![ptrT] "s")))) #());;;
+      let: "n" := ref_ty ptrT (zero_val ptrT) in
+      return: (ENotLeader, ![ptrT] "n", nil);;;
+      do:  #()
+    else do:  #());;;
+    let: "tryRelease" := ref_ty funcT (zero_val funcT) in
+    let: "$r0" := (λ: <>,
+      let: "$r0" := let: "$a0" := ![uint64T] (struct.field_ref paxosState "nextIndex" (![ptrT] (struct.field_ref Server "ps" (![ptrT] "s")))) in
+      let: "$a1" := #1 in
+      std.SumAssumeNoOverflow "$a0" "$a1" in
+      do:  ((struct.field_ref paxosState "nextIndex" (![ptrT] (struct.field_ref Server "ps" (![ptrT] "s")))) <-[uint64T] "$r0");;;
+      let: "args" := ref_ty ptrT (zero_val ptrT) in
+      let: "$r0" := ref_ty applyAsFollowerArgs (struct.make applyAsFollowerArgs [{
+        "epoch" ::= ![uint64T] (struct.field_ref paxosState "epoch" (![ptrT] (struct.field_ref Server "ps" (![ptrT] "s"))));
+        "nextIndex" ::= ![uint64T] (struct.field_ref paxosState "nextIndex" (![ptrT] (struct.field_ref Server "ps" (![ptrT] "s"))));
+        "state" ::= ![sliceT byteT] (struct.field_ref paxosState "state" (![ptrT] (struct.field_ref Server "ps" (![ptrT] "s"))))
+      }]) in
+      do:  ("args" <-[ptrT] "$r0");;;
+      let: "waitFn" := ref_ty funcT (zero_val funcT) in
+      let: "$r0" := let: "$a0" := let: "$a0" := ![ptrT] (struct.field_ref Server "ps" (![ptrT] "s")) in
+      encodePaxosState "$a0" in
+      (asyncfile.AsyncFile__Write (![ptrT] (struct.field_ref Server "storage" (![ptrT] "s")))) "$a0" in
+      do:  ("waitFn" <-[funcT] "$r0");;;
+      do:  ((sync.Mutex__Unlock (![ptrT] (struct.field_ref Server "mu" (![ptrT] "s")))) #());;;
+      do:  ((![funcT] "waitFn") #());;;
+      let: "clerks" := ref_ty (sliceT ptrT) (zero_val (sliceT ptrT)) in
+      let: "$r0" := ![sliceT ptrT] (struct.field_ref Server "clerks" (![ptrT] "s")) in
+      do:  ("clerks" <-[sliceT ptrT] "$r0");;;
+      let: "numReplies" := ref_ty uint64T #0 in
+      let: "replies" := ref_ty (sliceT ptrT) (zero_val (sliceT ptrT)) in
+      let: "$r0" := slice.make2 ptrT (slice.len (![sliceT ptrT] "clerks")) in
+      do:  ("replies" <-[sliceT ptrT] "$r0");;;
+      let: "mu" := ref_ty ptrT (zero_val ptrT) in
+      let: "$r0" := ref_ty sync.Mutex (zero_val sync.Mutex) in
+      do:  ("mu" <-[ptrT] "$r0");;;
+      let: "numReplies_cond" := ref_ty ptrT (zero_val ptrT) in
+      let: "$r0" := let: "$a0" := interface.make sync.Mutex__mset_ptr (![ptrT] "mu") in
+      sync.NewCond "$a0" in
+      do:  ("numReplies_cond" <-[ptrT] "$r0");;;
+      let: "n" := ref_ty uint64T (zero_val uint64T) in
+      let: "$r0" := slice.len (![sliceT ptrT] "clerks") in
+      do:  ("n" <-[uint64T] "$r0");;;
+      do:  (let: "$range" := ![sliceT ptrT] "clerks" in
+      slice.for_range ptrT "$range" (λ: "i" "ck",
+        let: "i" := ref_ty uint64T "i" in
+        let: "ck" := ref_ty ptrT "ck" in
+        let: "ck" := ref_ty ptrT (zero_val ptrT) in
+        let: "$r0" := ![ptrT] "ck" in
+        do:  ("ck" <-[ptrT] "$r0");;;
+        let: "i" := ref_ty intT (zero_val intT) in
+        let: "$r0" := ![intT] "i" in
+        do:  ("i" <-[intT] "$r0");;;
+        let: "$go" := (λ: <>,
+          let: "reply" := ref_ty ptrT (zero_val ptrT) in
+          let: "$r0" := let: "$a0" := ![ptrT] "args" in
+          (singleClerk__applyAsFollower (![ptrT] "ck")) "$a0" in
+          do:  ("reply" <-[ptrT] "$r0");;;
+          do:  ((sync.Mutex__Lock (![ptrT] "mu")) #());;;
+          do:  ("numReplies" <-[uint64T] ((![uint64T] "numReplies") + #1));;;
+          let: "$r0" := ![ptrT] "reply" in
+          do:  ((slice.elem_ref ptrT (![sliceT ptrT] "replies") (![intT] "i")) <-[ptrT] "$r0");;;
+          (if: (#2 * (![uint64T] "numReplies")) > (![uint64T] "n")
+          then
+            do:  ((sync.Cond__Signal (![ptrT] "numReplies_cond")) #());;;
+            do:  #()
+          else do:  #());;;
+          do:  ((sync.Mutex__Unlock (![ptrT] "mu")) #());;;
+          do:  #()
+          ) in
+        do:  (Fork ("$go" #()));;;
+        do:  #()));;;
+      do:  ((sync.Mutex__Lock (![ptrT] "mu")) #());;;
+      (for: (λ: <>, (#2 * (![uint64T] "numReplies")) ≤ (![uint64T] "n")); (λ: <>, Skip) := λ: <>,
+        do:  ((sync.Cond__Wait (![ptrT] "numReplies_cond")) #());;;
+        do:  #());;;
+      let: "numSuccesses" := ref_ty uint64T #0 in
+      do:  (let: "$range" := ![sliceT ptrT] "replies" in
+      slice.for_range ptrT "$range" (λ: <> "reply",
+        let: "reply" := ref_ty ptrT "reply" in
+        (if: (![ptrT] "reply") ≠ #null
+        then
+          (if: (![Error] (struct.field_ref applyAsFollowerReply "err" (![ptrT] "reply"))) = ENone
+          then
+            do:  ("numSuccesses" <-[uint64T] ((![uint64T] "numSuccesses") + #1));;;
+            do:  #()
+          else do:  #());;;
+          do:  #()
+        else do:  #());;;
+        do:  #()));;;
+      (if: (#2 * (![uint64T] "numSuccesses")) > (![uint64T] "n")
+      then
+        let: "$r0" := ENone in
+        do:  ("retErr" <-[Error] "$r0");;;
+        do:  #()
+      else
+        let: "$r0" := EEpochStale in
+        do:  ("retErr" <-[Error] "$r0");;;
+        do:  #());;;
+      return: (![Error] "retErr");;;
+      do:  #()
+      ) in
+    do:  ("tryRelease" <-[funcT] "$r0");;;
+    return: (ENone, struct.field_ref paxosState "state" (![ptrT] (struct.field_ref Server "ps" (![ptrT] "s"))), ![funcT] "tryRelease");;;
+    do:  #()).
+
+(* go: server.go:28:18 *)
 Definition Server__withLock : val :=
   rec: "Server__withLock" "s" "f" :=
     exception_do (let: "s" := ref_ty ptrT "s" in
     let: "f" := ref_ty funcT "f" in
-    do:  (sync.Mutex__Lock (![ptrT] (struct.field_ref Server "mu" (![ptrT] "s")))) #();;;
-    do:  (![funcT] "f") (![ptrT] (struct.field_ref Server "ps" (![ptrT] "s")));;;
+    do:  ((sync.Mutex__Lock (![ptrT] (struct.field_ref Server "mu" (![ptrT] "s")))) #());;;
+    do:  (let: "$a0" := ![ptrT] (struct.field_ref Server "ps" (![ptrT] "s")) in
+    (![funcT] "f") "$a0");;;
     let: "waitFn" := ref_ty funcT (zero_val funcT) in
-    let: "$a0" := (asyncfile.AsyncFile__Write (![ptrT] (struct.field_ref Server "storage" (![ptrT] "s")))) (encodePaxosState (![ptrT] (struct.field_ref Server "ps" (![ptrT] "s")))) in
-    do:  "waitFn" <-[funcT] "$a0";;;
-    do:  (sync.Mutex__Unlock (![ptrT] (struct.field_ref Server "mu" (![ptrT] "s")))) #();;;
-    do:  (![funcT] "waitFn") #();;;
+    let: "$r0" := let: "$a0" := let: "$a0" := ![ptrT] (struct.field_ref Server "ps" (![ptrT] "s")) in
+    encodePaxosState "$a0" in
+    (asyncfile.AsyncFile__Write (![ptrT] (struct.field_ref Server "storage" (![ptrT] "s")))) "$a0" in
+    do:  ("waitFn" <-[funcT] "$r0");;;
+    do:  ((sync.Mutex__Unlock (![ptrT] (struct.field_ref Server "mu" (![ptrT] "s")))) #());;;
+    do:  ((![funcT] "waitFn") #());;;
     do:  #()).
 
-Definition Server__applyAsFollower : val :=
-  rec: "Server__applyAsFollower" "s" "args" "reply" :=
-    exception_do (let: "s" := ref_ty ptrT "s" in
-    let: "reply" := ref_ty ptrT "reply" in
-    let: "args" := ref_ty ptrT "args" in
-    do:  (Server__withLock (![ptrT] "s")) (λ: "ps",
-      (if: (![uint64T] (struct.field_ref paxosState "epoch" (![ptrT] "ps"))) ≤ (![uint64T] (struct.field_ref applyAsFollowerArgs "epoch" (![ptrT] "args")))
-      then
-        (if: (![uint64T] (struct.field_ref paxosState "acceptedEpoch" (![ptrT] "ps"))) = (![uint64T] (struct.field_ref applyAsFollowerArgs "epoch" (![ptrT] "args")))
-        then
-          (if: (![uint64T] (struct.field_ref paxosState "nextIndex" (![ptrT] "ps"))) < (![uint64T] (struct.field_ref applyAsFollowerArgs "nextIndex" (![ptrT] "args")))
-          then
-            let: "$a0" := ![uint64T] (struct.field_ref applyAsFollowerArgs "nextIndex" (![ptrT] "args")) in
-            do:  (struct.field_ref paxosState "nextIndex" (![ptrT] "ps")) <-[uint64T] "$a0";;;
-            let: "$a0" := ![sliceT byteT] (struct.field_ref applyAsFollowerArgs "state" (![ptrT] "args")) in
-            do:  (struct.field_ref paxosState "state" (![ptrT] "ps")) <-[sliceT byteT] "$a0";;;
-            let: "$a0" := ENone in
-            do:  (struct.field_ref applyAsFollowerReply "err" (![ptrT] "reply")) <-[Error] "$a0";;;
-            do:  #()
-          else
-            let: "$a0" := ENone in
-            do:  (struct.field_ref applyAsFollowerReply "err" (![ptrT] "reply")) <-[Error] "$a0";;;
-            do:  #());;;
-          do:  #()
-        else
-          let: "$a0" := ![uint64T] (struct.field_ref applyAsFollowerArgs "epoch" (![ptrT] "args")) in
-          do:  (struct.field_ref paxosState "acceptedEpoch" (![ptrT] "ps")) <-[uint64T] "$a0";;;
-          let: "$a0" := ![uint64T] (struct.field_ref applyAsFollowerArgs "epoch" (![ptrT] "args")) in
-          do:  (struct.field_ref paxosState "epoch" (![ptrT] "ps")) <-[uint64T] "$a0";;;
-          let: "$a0" := ![sliceT byteT] (struct.field_ref applyAsFollowerArgs "state" (![ptrT] "args")) in
-          do:  (struct.field_ref paxosState "state" (![ptrT] "ps")) <-[sliceT byteT] "$a0";;;
-          let: "$a0" := ![uint64T] (struct.field_ref applyAsFollowerArgs "nextIndex" (![ptrT] "args")) in
-          do:  (struct.field_ref paxosState "nextIndex" (![ptrT] "ps")) <-[uint64T] "$a0";;;
-          let: "$a0" := #false in
-          do:  (struct.field_ref paxosState "isLeader" (![ptrT] "ps")) <-[boolT] "$a0";;;
-          let: "$a0" := ENone in
-          do:  (struct.field_ref applyAsFollowerReply "err" (![ptrT] "reply")) <-[Error] "$a0";;;
-          do:  #());;;
-        do:  #()
-      else
-        let: "$a0" := EEpochStale in
-        do:  (struct.field_ref applyAsFollowerReply "err" (![ptrT] "reply")) <-[Error] "$a0";;;
-        do:  #());;;
-      do:  #()
-      );;;
-    do:  #()).
-
-(* NOTE:
-   This will vote yes only the first time it's called in an epoch.
-   If you have too aggressive of a timeout and end up retrying this, the retry
-   might fail because it may be the second execution of enterNewEpoch(epoch) on
-   the server.
-   Solution: either conservative (maybe double) timeouts, or don't use this for
-   leader election, only for coming up with a valid proposal. *)
-Definition Server__enterNewEpoch : val :=
-  rec: "Server__enterNewEpoch" "s" "args" "reply" :=
-    exception_do (let: "s" := ref_ty ptrT "s" in
-    let: "reply" := ref_ty ptrT "reply" in
-    let: "args" := ref_ty ptrT "args" in
-    do:  (Server__withLock (![ptrT] "s")) (λ: "ps",
-      (if: (![uint64T] (struct.field_ref paxosState "epoch" (![ptrT] "ps"))) ≥ (![uint64T] (struct.field_ref enterNewEpochArgs "epoch" (![ptrT] "args")))
-      then
-        let: "$a0" := EEpochStale in
-        do:  (struct.field_ref enterNewEpochReply "err" (![ptrT] "reply")) <-[Error] "$a0";;;
-        return: (#());;;
-        do:  #()
-      else do:  #());;;
-      let: "$a0" := #false in
-      do:  (struct.field_ref paxosState "isLeader" (![ptrT] "ps")) <-[boolT] "$a0";;;
-      let: "$a0" := ![uint64T] (struct.field_ref enterNewEpochArgs "epoch" (![ptrT] "args")) in
-      do:  (struct.field_ref paxosState "epoch" (![ptrT] "ps")) <-[uint64T] "$a0";;;
-      let: "$a0" := ![uint64T] (struct.field_ref paxosState "acceptedEpoch" (![ptrT] "ps")) in
-      do:  (struct.field_ref enterNewEpochReply "acceptedEpoch" (![ptrT] "reply")) <-[uint64T] "$a0";;;
-      let: "$a0" := ![uint64T] (struct.field_ref paxosState "nextIndex" (![ptrT] "ps")) in
-      do:  (struct.field_ref enterNewEpochReply "nextIndex" (![ptrT] "reply")) <-[uint64T] "$a0";;;
-      let: "$a0" := ![sliceT byteT] (struct.field_ref paxosState "state" (![ptrT] "ps")) in
-      do:  (struct.field_ref enterNewEpochReply "state" (![ptrT] "reply")) <-[sliceT byteT] "$a0";;;
-      do:  #()
-      );;;
-    do:  #()).
-
+(* go: server.go:83:18 *)
 Definition Server__TryBecomeLeader : val :=
   rec: "Server__TryBecomeLeader" "s" <> :=
     exception_do (let: "s" := ref_ty ptrT "s" in
-    do:  log.Println #(str "started trybecomeleader");;;
-    do:  (sync.Mutex__Lock (![ptrT] (struct.field_ref Server "mu" (![ptrT] "s")))) #();;;
+    do:  (let: "$a0" := (let: "$sl0" := interface.make string__mset #(str "started trybecomeleader") in
+    slice.literal ["$sl0"]) in
+    log.Println "$a0");;;
+    do:  ((sync.Mutex__Lock (![ptrT] (struct.field_ref Server "mu" (![ptrT] "s")))) #());;;
     (if: ![boolT] (struct.field_ref paxosState "isLeader" (![ptrT] (struct.field_ref Server "ps" (![ptrT] "s"))))
     then
-      do:  log.Println #(str "already leader");;;
-      do:  (sync.Mutex__Unlock (![ptrT] (struct.field_ref Server "mu" (![ptrT] "s")))) #();;;
+      do:  (let: "$a0" := (let: "$sl0" := interface.make string__mset #(str "already leader") in
+      slice.literal ["$sl0"]) in
+      log.Println "$a0");;;
+      do:  ((sync.Mutex__Unlock (![ptrT] (struct.field_ref Server "mu" (![ptrT] "s")))) #());;;
       return: (#());;;
       do:  #()
     else do:  #());;;
     let: "clerks" := ref_ty (sliceT ptrT) (zero_val (sliceT ptrT)) in
-    let: "$a0" := ![sliceT ptrT] (struct.field_ref Server "clerks" (![ptrT] "s")) in
-    do:  "clerks" <-[sliceT ptrT] "$a0";;;
+    let: "$r0" := ![sliceT ptrT] (struct.field_ref Server "clerks" (![ptrT] "s")) in
+    do:  ("clerks" <-[sliceT ptrT] "$r0");;;
     let: "args" := ref_ty ptrT (zero_val ptrT) in
-    let: "$a0" := ref_ty enterNewEpochArgs (struct.make enterNewEpochArgs [{
+    let: "$r0" := ref_ty enterNewEpochArgs (struct.make enterNewEpochArgs [{
       "epoch" ::= (![uint64T] (struct.field_ref paxosState "epoch" (![ptrT] (struct.field_ref Server "ps" (![ptrT] "s"))))) + #1
     }]) in
-    do:  "args" <-[ptrT] "$a0";;;
-    do:  (sync.Mutex__Unlock (![ptrT] (struct.field_ref Server "mu" (![ptrT] "s")))) #();;;
+    do:  ("args" <-[ptrT] "$r0");;;
+    do:  ((sync.Mutex__Unlock (![ptrT] (struct.field_ref Server "mu" (![ptrT] "s")))) #());;;
     let: "numReplies" := ref_ty uint64T #0 in
     let: "replies" := ref_ty (sliceT ptrT) (zero_val (sliceT ptrT)) in
-    let: "$a0" := slice.make2 ptrT (slice.len (![sliceT ptrT] "clerks")) in
-    do:  "replies" <-[sliceT ptrT] "$a0";;;
+    let: "$r0" := slice.make2 ptrT (slice.len (![sliceT ptrT] "clerks")) in
+    do:  ("replies" <-[sliceT ptrT] "$r0");;;
     let: "mu" := ref_ty ptrT (zero_val ptrT) in
-    let: "$a0" := ref_ty sync.Mutex (zero_val sync.Mutex) in
-    do:  "mu" <-[ptrT] "$a0";;;
+    let: "$r0" := ref_ty sync.Mutex (zero_val sync.Mutex) in
+    do:  ("mu" <-[ptrT] "$r0");;;
     let: "numReplies_cond" := ref_ty ptrT (zero_val ptrT) in
-    let: "$a0" := sync.NewCond (![ptrT] "mu") in
-    do:  "numReplies_cond" <-[ptrT] "$a0";;;
+    let: "$r0" := let: "$a0" := interface.make sync.Mutex__mset_ptr (![ptrT] "mu") in
+    sync.NewCond "$a0" in
+    do:  ("numReplies_cond" <-[ptrT] "$r0");;;
     let: "n" := ref_ty uint64T (zero_val uint64T) in
-    let: "$a0" := slice.len (![sliceT ptrT] "clerks") in
-    do:  "n" <-[uint64T] "$a0";;;
-    do:  let: "$range" := ![sliceT ptrT] "clerks" in
+    let: "$r0" := slice.len (![sliceT ptrT] "clerks") in
+    do:  ("n" <-[uint64T] "$r0");;;
+    do:  (let: "$range" := ![sliceT ptrT] "clerks" in
     slice.for_range ptrT "$range" (λ: "i" "ck",
       let: "i" := ref_ty uint64T "i" in
       let: "ck" := ref_ty ptrT "ck" in
       let: "$go" := (λ: <>,
         let: "reply" := ref_ty ptrT (zero_val ptrT) in
-        let: "$a0" := (singleClerk__enterNewEpoch (![ptrT] "ck")) (![ptrT] "args") in
-        do:  "reply" <-[ptrT] "$a0";;;
-        do:  (sync.Mutex__Lock (![ptrT] "mu")) #();;;
-        do:  "numReplies" <-[uint64T] ((![uint64T] "numReplies") + #1);;;
-        let: "$a0" := ![ptrT] "reply" in
-        do:  (slice.elem_ref ptrT (![sliceT ptrT] "replies") (![intT] "i")) <-[ptrT] "$a0";;;
+        let: "$r0" := let: "$a0" := ![ptrT] "args" in
+        (singleClerk__enterNewEpoch (![ptrT] "ck")) "$a0" in
+        do:  ("reply" <-[ptrT] "$r0");;;
+        do:  ((sync.Mutex__Lock (![ptrT] "mu")) #());;;
+        do:  ("numReplies" <-[uint64T] ((![uint64T] "numReplies") + #1));;;
+        let: "$r0" := ![ptrT] "reply" in
+        do:  ((slice.elem_ref ptrT (![sliceT ptrT] "replies") (![intT] "i")) <-[ptrT] "$r0");;;
         (if: (#2 * (![uint64T] "numReplies")) > (![uint64T] "n")
         then
-          do:  (sync.Cond__Signal (![ptrT] "numReplies_cond")) #();;;
+          do:  ((sync.Cond__Signal (![ptrT] "numReplies_cond")) #());;;
           do:  #()
         else do:  #());;;
-        do:  (sync.Mutex__Unlock (![ptrT] "mu")) #();;;
+        do:  ((sync.Mutex__Unlock (![ptrT] "mu")) #());;;
         do:  #()
         ) in
-      do:  Fork ("$go" #());;;
-      do:  #());;;
-    do:  (sync.Mutex__Lock (![ptrT] "mu")) #();;;
+      do:  (Fork ("$go" #()));;;
+      do:  #()));;;
+    do:  ((sync.Mutex__Lock (![ptrT] "mu")) #());;;
     (for: (λ: <>, (#2 * (![uint64T] "numReplies")) ≤ (![uint64T] "n")); (λ: <>, Skip) := λ: <>,
-      do:  (sync.Cond__Wait (![ptrT] "numReplies_cond")) #();;;
+      do:  ((sync.Cond__Wait (![ptrT] "numReplies_cond")) #());;;
       do:  #());;;
     let: "latestReply" := ref_ty ptrT (zero_val ptrT) in
     let: "numSuccesses" := ref_ty uint64T #0 in
-    do:  let: "$range" := ![sliceT ptrT] "replies" in
+    do:  (let: "$range" := ![sliceT ptrT] "replies" in
     slice.for_range ptrT "$range" (λ: <> "reply",
       let: "reply" := ref_ty ptrT "reply" in
       (if: (![ptrT] "reply") ≠ #null
@@ -526,212 +716,215 @@ Definition Server__TryBecomeLeader : val :=
         then
           (if: (![uint64T] "numSuccesses") = #0
           then
-            let: "$a0" := ![ptrT] "reply" in
-            do:  "latestReply" <-[ptrT] "$a0";;;
+            let: "$r0" := ![ptrT] "reply" in
+            do:  ("latestReply" <-[ptrT] "$r0");;;
             do:  #()
           else
             (if: (![uint64T] (struct.field_ref enterNewEpochReply "acceptedEpoch" (![ptrT] "latestReply"))) < (![uint64T] (struct.field_ref enterNewEpochReply "acceptedEpoch" (![ptrT] "reply")))
             then
-              let: "$a0" := ![ptrT] "reply" in
-              do:  "latestReply" <-[ptrT] "$a0";;;
+              let: "$r0" := ![ptrT] "reply" in
+              do:  ("latestReply" <-[ptrT] "$r0");;;
               do:  #()
             else
               (if: ((![uint64T] (struct.field_ref enterNewEpochReply "acceptedEpoch" (![ptrT] "latestReply"))) = (![uint64T] (struct.field_ref enterNewEpochReply "acceptedEpoch" (![ptrT] "reply")))) && ((![uint64T] (struct.field_ref enterNewEpochReply "nextIndex" (![ptrT] "reply"))) > (![uint64T] (struct.field_ref enterNewEpochReply "nextIndex" (![ptrT] "latestReply"))))
               then
-                let: "$a0" := ![ptrT] "reply" in
-                do:  "latestReply" <-[ptrT] "$a0";;;
+                let: "$r0" := ![ptrT] "reply" in
+                do:  ("latestReply" <-[ptrT] "$r0");;;
                 do:  #()
               else do:  #());;;
               #());;;
             do:  #());;;
-          do:  "numSuccesses" <-[uint64T] ((![uint64T] "numSuccesses") + #1);;;
+          do:  ("numSuccesses" <-[uint64T] ((![uint64T] "numSuccesses") + #1));;;
           do:  #()
         else do:  #());;;
         do:  #()
       else do:  #());;;
-      do:  #());;;
+      do:  #()));;;
     (if: (#2 * (![uint64T] "numSuccesses")) > (![uint64T] "n")
     then
-      do:  (Server__withLock (![ptrT] "s")) (λ: "ps",
+      do:  (let: "$a0" := (λ: "ps",
         (if: (![uint64T] (struct.field_ref paxosState "epoch" (![ptrT] "ps"))) ≤ (![uint64T] (struct.field_ref enterNewEpochArgs "epoch" (![ptrT] "args")))
         then
-          do:  log.Printf #(str "succeeded becomeleader in epoch %!!(MISSING)!(MISSING)!(MISSING)!(MISSING)!(MISSING)!(MISSING)!(MISSING)!(MISSING)!(MISSING)!(MISSING)!(MISSING)!(MISSING)!(MISSING)!(MISSING)!(MISSING)!(MISSING)!(MISSING)!(MISSING)!(MISSING)!(MISSING)!(MISSING)!(MISSING)!(MISSING)!(MISSING)!(MISSING)!(MISSING)!(MISSING)!(MISSING)!(MISSING)d(MISSING)
-          ") (![uint64T] (struct.field_ref enterNewEpochArgs "epoch" (![ptrT] "args")));;;
-          let: "$a0" := ![uint64T] (struct.field_ref enterNewEpochArgs "epoch" (![ptrT] "args")) in
-          do:  (struct.field_ref paxosState "epoch" (![ptrT] "ps")) <-[uint64T] "$a0";;;
-          let: "$a0" := #true in
-          do:  (struct.field_ref paxosState "isLeader" (![ptrT] "ps")) <-[boolT] "$a0";;;
-          let: "$a0" := ![uint64T] (struct.field_ref paxosState "epoch" (![ptrT] "ps")) in
-          do:  (struct.field_ref paxosState "acceptedEpoch" (![ptrT] "ps")) <-[uint64T] "$a0";;;
-          let: "$a0" := ![uint64T] (struct.field_ref enterNewEpochReply "nextIndex" (![ptrT] "latestReply")) in
-          do:  (struct.field_ref paxosState "nextIndex" (![ptrT] "ps")) <-[uint64T] "$a0";;;
-          let: "$a0" := ![sliceT byteT] (struct.field_ref enterNewEpochReply "state" (![ptrT] "latestReply")) in
-          do:  (struct.field_ref paxosState "state" (![ptrT] "ps")) <-[sliceT byteT] "$a0";;;
+          do:  (let: "$a0" := #(str "succeeded becomeleader in epoch %d
+          ") in
+          let: "$a1" := (let: "$sl0" := interface.make uint64__mset (![uint64T] (struct.field_ref enterNewEpochArgs "epoch" (![ptrT] "args"))) in
+          slice.literal ["$sl0"]) in
+          log.Printf "$a0" "$a1");;;
+          let: "$r0" := ![uint64T] (struct.field_ref enterNewEpochArgs "epoch" (![ptrT] "args")) in
+          do:  ((struct.field_ref paxosState "epoch" (![ptrT] "ps")) <-[uint64T] "$r0");;;
+          let: "$r0" := #true in
+          do:  ((struct.field_ref paxosState "isLeader" (![ptrT] "ps")) <-[boolT] "$r0");;;
+          let: "$r0" := ![uint64T] (struct.field_ref paxosState "epoch" (![ptrT] "ps")) in
+          do:  ((struct.field_ref paxosState "acceptedEpoch" (![ptrT] "ps")) <-[uint64T] "$r0");;;
+          let: "$r0" := ![uint64T] (struct.field_ref enterNewEpochReply "nextIndex" (![ptrT] "latestReply")) in
+          do:  ((struct.field_ref paxosState "nextIndex" (![ptrT] "ps")) <-[uint64T] "$r0");;;
+          let: "$r0" := ![sliceT byteT] (struct.field_ref enterNewEpochReply "state" (![ptrT] "latestReply")) in
+          do:  ((struct.field_ref paxosState "state" (![ptrT] "ps")) <-[sliceT byteT] "$r0");;;
           do:  #()
         else do:  #());;;
         do:  #()
-        );;;
-      do:  (sync.Mutex__Unlock (![ptrT] "mu")) #();;;
+        ) in
+      (Server__withLock (![ptrT] "s")) "$a0");;;
+      do:  ((sync.Mutex__Unlock (![ptrT] "mu")) #());;;
       do:  #()
     else
-      do:  (sync.Mutex__Unlock (![ptrT] "mu")) #();;;
-      do:  log.Println #(str "failed becomeleader");;;
+      do:  ((sync.Mutex__Unlock (![ptrT] "mu")) #());;;
+      do:  (let: "$a0" := (let: "$sl0" := interface.make string__mset #(str "failed becomeleader") in
+      slice.literal ["$sl0"]) in
+      log.Println "$a0");;;
       do:  #());;;
     do:  #()).
 
-Definition Server__TryAcquire : val :=
-  rec: "Server__TryAcquire" "s" <> :=
-    exception_do (let: "s" := ref_ty ptrT "s" in
-    let: "retErr" := ref_ty Error (zero_val Error) in
-    do:  (sync.Mutex__Lock (![ptrT] (struct.field_ref Server "mu" (![ptrT] "s")))) #();;;
-    (if: (~ (![boolT] (struct.field_ref paxosState "isLeader" (![ptrT] (struct.field_ref Server "ps" (![ptrT] "s"))))))
-    then
-      do:  (sync.Mutex__Unlock (![ptrT] (struct.field_ref Server "mu" (![ptrT] "s")))) #();;;
-      let: "n" := ref_ty ptrT (zero_val ptrT) in
-      return: (ENotLeader, ![ptrT] "n", slice.nil);;;
-      do:  #()
-    else do:  #());;;
-    let: "tryRelease" := ref_ty funcT (zero_val funcT) in
-    let: "$a0" := (λ: <>,
-      let: "$a0" := std.SumAssumeNoOverflow (![uint64T] (struct.field_ref paxosState "nextIndex" (![ptrT] (struct.field_ref Server "ps" (![ptrT] "s"))))) #1 in
-      do:  (struct.field_ref paxosState "nextIndex" (![ptrT] (struct.field_ref Server "ps" (![ptrT] "s")))) <-[uint64T] "$a0";;;
-      let: "args" := ref_ty ptrT (zero_val ptrT) in
-      let: "$a0" := ref_ty applyAsFollowerArgs (struct.make applyAsFollowerArgs [{
-        "epoch" ::= ![uint64T] (struct.field_ref paxosState "epoch" (![ptrT] (struct.field_ref Server "ps" (![ptrT] "s"))));
-        "nextIndex" ::= ![uint64T] (struct.field_ref paxosState "nextIndex" (![ptrT] (struct.field_ref Server "ps" (![ptrT] "s"))));
-        "state" ::= ![sliceT byteT] (struct.field_ref paxosState "state" (![ptrT] (struct.field_ref Server "ps" (![ptrT] "s"))))
-      }]) in
-      do:  "args" <-[ptrT] "$a0";;;
-      let: "waitFn" := ref_ty funcT (zero_val funcT) in
-      let: "$a0" := (asyncfile.AsyncFile__Write (![ptrT] (struct.field_ref Server "storage" (![ptrT] "s")))) (encodePaxosState (![ptrT] (struct.field_ref Server "ps" (![ptrT] "s")))) in
-      do:  "waitFn" <-[funcT] "$a0";;;
-      do:  (sync.Mutex__Unlock (![ptrT] (struct.field_ref Server "mu" (![ptrT] "s")))) #();;;
-      do:  (![funcT] "waitFn") #();;;
-      let: "clerks" := ref_ty (sliceT ptrT) (zero_val (sliceT ptrT)) in
-      let: "$a0" := ![sliceT ptrT] (struct.field_ref Server "clerks" (![ptrT] "s")) in
-      do:  "clerks" <-[sliceT ptrT] "$a0";;;
-      let: "numReplies" := ref_ty uint64T #0 in
-      let: "replies" := ref_ty (sliceT ptrT) (zero_val (sliceT ptrT)) in
-      let: "$a0" := slice.make2 ptrT (slice.len (![sliceT ptrT] "clerks")) in
-      do:  "replies" <-[sliceT ptrT] "$a0";;;
-      let: "mu" := ref_ty ptrT (zero_val ptrT) in
-      let: "$a0" := ref_ty sync.Mutex (zero_val sync.Mutex) in
-      do:  "mu" <-[ptrT] "$a0";;;
-      let: "numReplies_cond" := ref_ty ptrT (zero_val ptrT) in
-      let: "$a0" := sync.NewCond (![ptrT] "mu") in
-      do:  "numReplies_cond" <-[ptrT] "$a0";;;
-      let: "n" := ref_ty uint64T (zero_val uint64T) in
-      let: "$a0" := slice.len (![sliceT ptrT] "clerks") in
-      do:  "n" <-[uint64T] "$a0";;;
-      do:  let: "$range" := ![sliceT ptrT] "clerks" in
-      slice.for_range ptrT "$range" (λ: "i" "ck",
-        let: "i" := ref_ty uint64T "i" in
-        let: "ck" := ref_ty ptrT "ck" in
-        let: "ck" := ref_ty ptrT (zero_val ptrT) in
-        let: "$a0" := ![ptrT] "ck" in
-        do:  "ck" <-[ptrT] "$a0";;;
-        let: "i" := ref_ty intT (zero_val intT) in
-        let: "$a0" := ![intT] "i" in
-        do:  "i" <-[intT] "$a0";;;
-        let: "$go" := (λ: <>,
-          let: "reply" := ref_ty ptrT (zero_val ptrT) in
-          let: "$a0" := (singleClerk__applyAsFollower (![ptrT] "ck")) (![ptrT] "args") in
-          do:  "reply" <-[ptrT] "$a0";;;
-          do:  (sync.Mutex__Lock (![ptrT] "mu")) #();;;
-          do:  "numReplies" <-[uint64T] ((![uint64T] "numReplies") + #1);;;
-          let: "$a0" := ![ptrT] "reply" in
-          do:  (slice.elem_ref ptrT (![sliceT ptrT] "replies") (![intT] "i")) <-[ptrT] "$a0";;;
-          (if: (#2 * (![uint64T] "numReplies")) > (![uint64T] "n")
-          then
-            do:  (sync.Cond__Signal (![ptrT] "numReplies_cond")) #();;;
-            do:  #()
-          else do:  #());;;
-          do:  (sync.Mutex__Unlock (![ptrT] "mu")) #();;;
-          do:  #()
-          ) in
-        do:  Fork ("$go" #());;;
-        do:  #());;;
-      do:  (sync.Mutex__Lock (![ptrT] "mu")) #();;;
-      (for: (λ: <>, (#2 * (![uint64T] "numReplies")) ≤ (![uint64T] "n")); (λ: <>, Skip) := λ: <>,
-        do:  (sync.Cond__Wait (![ptrT] "numReplies_cond")) #();;;
-        do:  #());;;
-      let: "numSuccesses" := ref_ty uint64T #0 in
-      do:  let: "$range" := ![sliceT ptrT] "replies" in
-      slice.for_range ptrT "$range" (λ: <> "reply",
-        let: "reply" := ref_ty ptrT "reply" in
-        (if: (![ptrT] "reply") ≠ #null
-        then
-          (if: (![Error] (struct.field_ref applyAsFollowerReply "err" (![ptrT] "reply"))) = ENone
-          then
-            do:  "numSuccesses" <-[uint64T] ((![uint64T] "numSuccesses") + #1);;;
-            do:  #()
-          else do:  #());;;
-          do:  #()
-        else do:  #());;;
-        do:  #());;;
-      (if: (#2 * (![uint64T] "numSuccesses")) > (![uint64T] "n")
-      then
-        let: "$a0" := ENone in
-        do:  "retErr" <-[Error] "$a0";;;
-        do:  #()
-      else
-        let: "$a0" := EEpochStale in
-        do:  "retErr" <-[Error] "$a0";;;
-        do:  #());;;
-      return: (![Error] "retErr");;;
-      do:  #()
-      ) in
-    do:  "tryRelease" <-[funcT] "$a0";;;
-    return: (ENone, struct.field_ref paxosState "state" (![ptrT] (struct.field_ref Server "ps" (![ptrT] "s"))), ![funcT] "tryRelease");;;
-    do:  #()).
-
+(* go: server.go:235:18 *)
 Definition Server__WeakRead : val :=
   rec: "Server__WeakRead" "s" <> :=
     exception_do (let: "s" := ref_ty ptrT "s" in
-    do:  (sync.Mutex__Lock (![ptrT] (struct.field_ref Server "mu" (![ptrT] "s")))) #();;;
+    do:  ((sync.Mutex__Lock (![ptrT] (struct.field_ref Server "mu" (![ptrT] "s")))) #());;;
     let: "ret" := ref_ty (sliceT byteT) (zero_val (sliceT byteT)) in
-    let: "$a0" := ![sliceT byteT] (struct.field_ref paxosState "state" (![ptrT] (struct.field_ref Server "ps" (![ptrT] "s")))) in
-    do:  "ret" <-[sliceT byteT] "$a0";;;
-    do:  (sync.Mutex__Unlock (![ptrT] (struct.field_ref Server "mu" (![ptrT] "s")))) #();;;
+    let: "$r0" := ![sliceT byteT] (struct.field_ref paxosState "state" (![ptrT] (struct.field_ref Server "ps" (![ptrT] "s")))) in
+    do:  ("ret" <-[sliceT byteT] "$r0");;;
+    do:  ((sync.Mutex__Unlock (![ptrT] (struct.field_ref Server "mu" (![ptrT] "s")))) #());;;
     return: (![sliceT byteT] "ret");;;
     do:  #()).
 
+(* go: server.go:36:18 *)
+Definition Server__applyAsFollower : val :=
+  rec: "Server__applyAsFollower" "s" "args" "reply" :=
+    exception_do (let: "s" := ref_ty ptrT "s" in
+    let: "reply" := ref_ty ptrT "reply" in
+    let: "args" := ref_ty ptrT "args" in
+    do:  (let: "$a0" := (λ: "ps",
+      (if: (![uint64T] (struct.field_ref paxosState "epoch" (![ptrT] "ps"))) ≤ (![uint64T] (struct.field_ref applyAsFollowerArgs "epoch" (![ptrT] "args")))
+      then
+        (if: (![uint64T] (struct.field_ref paxosState "acceptedEpoch" (![ptrT] "ps"))) = (![uint64T] (struct.field_ref applyAsFollowerArgs "epoch" (![ptrT] "args")))
+        then
+          (if: (![uint64T] (struct.field_ref paxosState "nextIndex" (![ptrT] "ps"))) < (![uint64T] (struct.field_ref applyAsFollowerArgs "nextIndex" (![ptrT] "args")))
+          then
+            let: "$r0" := ![uint64T] (struct.field_ref applyAsFollowerArgs "nextIndex" (![ptrT] "args")) in
+            do:  ((struct.field_ref paxosState "nextIndex" (![ptrT] "ps")) <-[uint64T] "$r0");;;
+            let: "$r0" := ![sliceT byteT] (struct.field_ref applyAsFollowerArgs "state" (![ptrT] "args")) in
+            do:  ((struct.field_ref paxosState "state" (![ptrT] "ps")) <-[sliceT byteT] "$r0");;;
+            let: "$r0" := ENone in
+            do:  ((struct.field_ref applyAsFollowerReply "err" (![ptrT] "reply")) <-[Error] "$r0");;;
+            do:  #()
+          else
+            let: "$r0" := ENone in
+            do:  ((struct.field_ref applyAsFollowerReply "err" (![ptrT] "reply")) <-[Error] "$r0");;;
+            do:  #());;;
+          do:  #()
+        else
+          let: "$r0" := ![uint64T] (struct.field_ref applyAsFollowerArgs "epoch" (![ptrT] "args")) in
+          do:  ((struct.field_ref paxosState "acceptedEpoch" (![ptrT] "ps")) <-[uint64T] "$r0");;;
+          let: "$r0" := ![uint64T] (struct.field_ref applyAsFollowerArgs "epoch" (![ptrT] "args")) in
+          do:  ((struct.field_ref paxosState "epoch" (![ptrT] "ps")) <-[uint64T] "$r0");;;
+          let: "$r0" := ![sliceT byteT] (struct.field_ref applyAsFollowerArgs "state" (![ptrT] "args")) in
+          do:  ((struct.field_ref paxosState "state" (![ptrT] "ps")) <-[sliceT byteT] "$r0");;;
+          let: "$r0" := ![uint64T] (struct.field_ref applyAsFollowerArgs "nextIndex" (![ptrT] "args")) in
+          do:  ((struct.field_ref paxosState "nextIndex" (![ptrT] "ps")) <-[uint64T] "$r0");;;
+          let: "$r0" := #false in
+          do:  ((struct.field_ref paxosState "isLeader" (![ptrT] "ps")) <-[boolT] "$r0");;;
+          let: "$r0" := ENone in
+          do:  ((struct.field_ref applyAsFollowerReply "err" (![ptrT] "reply")) <-[Error] "$r0");;;
+          do:  #());;;
+        do:  #()
+      else
+        let: "$r0" := EEpochStale in
+        do:  ((struct.field_ref applyAsFollowerReply "err" (![ptrT] "reply")) <-[Error] "$r0");;;
+        do:  #());;;
+      do:  #()
+      ) in
+    (Server__withLock (![ptrT] "s")) "$a0");;;
+    do:  #()).
+
+(* NOTE:
+   This will vote yes only the first time it's called in an epoch.
+   If you have too aggressive of a timeout and end up retrying this, the retry
+   might fail because it may be the second execution of enterNewEpoch(epoch) on
+   the server.
+   Solution: either conservative (maybe double) timeouts, or don't use this for
+   leader election, only for coming up with a valid proposal.
+
+   go: server.go:68:18 *)
+Definition Server__enterNewEpoch : val :=
+  rec: "Server__enterNewEpoch" "s" "args" "reply" :=
+    exception_do (let: "s" := ref_ty ptrT "s" in
+    let: "reply" := ref_ty ptrT "reply" in
+    let: "args" := ref_ty ptrT "args" in
+    do:  (let: "$a0" := (λ: "ps",
+      (if: (![uint64T] (struct.field_ref paxosState "epoch" (![ptrT] "ps"))) ≥ (![uint64T] (struct.field_ref enterNewEpochArgs "epoch" (![ptrT] "args")))
+      then
+        let: "$r0" := EEpochStale in
+        do:  ((struct.field_ref enterNewEpochReply "err" (![ptrT] "reply")) <-[Error] "$r0");;;
+        return: (#());;;
+        do:  #()
+      else do:  #());;;
+      let: "$r0" := #false in
+      do:  ((struct.field_ref paxosState "isLeader" (![ptrT] "ps")) <-[boolT] "$r0");;;
+      let: "$r0" := ![uint64T] (struct.field_ref enterNewEpochArgs "epoch" (![ptrT] "args")) in
+      do:  ((struct.field_ref paxosState "epoch" (![ptrT] "ps")) <-[uint64T] "$r0");;;
+      let: "$r0" := ![uint64T] (struct.field_ref paxosState "acceptedEpoch" (![ptrT] "ps")) in
+      do:  ((struct.field_ref enterNewEpochReply "acceptedEpoch" (![ptrT] "reply")) <-[uint64T] "$r0");;;
+      let: "$r0" := ![uint64T] (struct.field_ref paxosState "nextIndex" (![ptrT] "ps")) in
+      do:  ((struct.field_ref enterNewEpochReply "nextIndex" (![ptrT] "reply")) <-[uint64T] "$r0");;;
+      let: "$r0" := ![sliceT byteT] (struct.field_ref paxosState "state" (![ptrT] "ps")) in
+      do:  ((struct.field_ref enterNewEpochReply "state" (![ptrT] "reply")) <-[sliceT byteT] "$r0");;;
+      do:  #()
+      ) in
+    (Server__withLock (![ptrT] "s")) "$a0");;;
+    do:  #()).
+
+Definition Server__mset_ptr : list (string * val) := [
+  ("TryAcquire", Server__TryAcquire);
+  ("TryBecomeLeader", Server__TryBecomeLeader);
+  ("WeakRead", Server__WeakRead);
+  ("applyAsFollower", Server__applyAsFollower);
+  ("enterNewEpoch", Server__enterNewEpoch);
+  ("withLock", Server__withLock)
+].
+
+(* go: server.go:242:6 *)
 Definition makeServer : val :=
   rec: "makeServer" "fname" "initstate" "config" :=
     exception_do (let: "config" := ref_ty (sliceT uint64T) "config" in
     let: "initstate" := ref_ty (sliceT byteT) "initstate" in
     let: "fname" := ref_ty stringT "fname" in
     let: "s" := ref_ty ptrT (zero_val ptrT) in
-    let: "$a0" := ref_ty Server (zero_val Server) in
-    do:  "s" <-[ptrT] "$a0";;;
-    let: "$a0" := ref_ty sync.Mutex (zero_val sync.Mutex) in
-    do:  (struct.field_ref Server "mu" (![ptrT] "s")) <-[ptrT] "$a0";;;
-    let: "$a0" := slice.make2 ptrT #0 in
-    do:  (struct.field_ref Server "clerks" (![ptrT] "s")) <-[sliceT ptrT] "$a0";;;
-    do:  let: "$range" := ![sliceT uint64T] "config" in
+    let: "$r0" := ref_ty Server (zero_val Server) in
+    do:  ("s" <-[ptrT] "$r0");;;
+    let: "$r0" := ref_ty sync.Mutex (zero_val sync.Mutex) in
+    do:  ((struct.field_ref Server "mu" (![ptrT] "s")) <-[ptrT] "$r0");;;
+    let: "$r0" := slice.make2 ptrT #0 in
+    do:  ((struct.field_ref Server "clerks" (![ptrT] "s")) <-[sliceT ptrT] "$r0");;;
+    do:  (let: "$range" := ![sliceT uint64T] "config" in
     slice.for_range uint64T "$range" (λ: <> "host",
       let: "host" := ref_ty uint64T "host" in
-      let: "$a0" := slice.append ptrT (![sliceT ptrT] (struct.field_ref Server "clerks" (![ptrT] "s"))) (slice.literal ptrT [MakeSingleClerk (![uint64T] "host")]) in
-      do:  (struct.field_ref Server "clerks" (![ptrT] "s")) <-[sliceT ptrT] "$a0";;;
-      do:  #());;;
+      let: "$r0" := slice.append ptrT (![sliceT ptrT] (struct.field_ref Server "clerks" (![ptrT] "s"))) (slice.literal ptrT [let: "$a0" := ![uint64T] "host" in
+       MakeSingleClerk "$a0"]) in
+      do:  ((struct.field_ref Server "clerks" (![ptrT] "s")) <-[sliceT ptrT] "$r0");;;
+      do:  #()));;;
     let: "encstate" := ref_ty (sliceT byteT) (zero_val (sliceT byteT)) in
-    let: ("$a0", "$a1") := asyncfile.MakeAsyncFile (![stringT] "fname") in
-    do:  (struct.field_ref Server "storage" (![ptrT] "s")) <-[ptrT] "$a1";;;
-    do:  "encstate" <-[sliceT byteT] "$a0";;;
+    let: ("$ret0", "$ret1") := let: "$a0" := ![stringT] "fname" in
+    asyncfile.MakeAsyncFile "$a0" in
+    let: "$r0" := "$ret0" in
+    let: "$r1" := "$ret1" in
+    do:  ("encstate" <-[sliceT byteT] "$r0");;;
+    do:  ((struct.field_ref Server "storage" (![ptrT] "s")) <-[ptrT] "$r1");;;
     (if: (slice.len (![sliceT byteT] "encstate")) = #0
     then
-      let: "$a0" := ref_ty paxosState (zero_val paxosState) in
-      do:  (struct.field_ref Server "ps" (![ptrT] "s")) <-[ptrT] "$a0";;;
-      let: "$a0" := ![sliceT byteT] "initstate" in
-      do:  (struct.field_ref paxosState "state" (![ptrT] (struct.field_ref Server "ps" (![ptrT] "s")))) <-[sliceT byteT] "$a0";;;
+      let: "$r0" := ref_ty paxosState (zero_val paxosState) in
+      do:  ((struct.field_ref Server "ps" (![ptrT] "s")) <-[ptrT] "$r0");;;
+      let: "$r0" := ![sliceT byteT] "initstate" in
+      do:  ((struct.field_ref paxosState "state" (![ptrT] (struct.field_ref Server "ps" (![ptrT] "s")))) <-[sliceT byteT] "$r0");;;
       do:  #()
     else
-      let: "$a0" := decodePaxosState (![sliceT byteT] "encstate") in
-      do:  (struct.field_ref Server "ps" (![ptrT] "s")) <-[ptrT] "$a0";;;
+      let: "$r0" := let: "$a0" := ![sliceT byteT] "encstate" in
+      decodePaxosState "$a0" in
+      do:  ((struct.field_ref Server "ps" (![ptrT] "s")) <-[ptrT] "$r0");;;
       do:  #());;;
     return: (![ptrT] "s");;;
     do:  #()).
 
+(* go: server.go:262:6 *)
 Definition StartServer : val :=
   rec: "StartServer" "fname" "initstate" "me" "config" :=
     exception_do (let: "config" := ref_ty (sliceT uint64T) "config" in
@@ -739,45 +932,58 @@ Definition StartServer : val :=
     let: "initstate" := ref_ty (sliceT byteT) "initstate" in
     let: "fname" := ref_ty stringT "fname" in
     let: "s" := ref_ty ptrT (zero_val ptrT) in
-    let: "$a0" := makeServer (![stringT] "fname") (![sliceT byteT] "initstate") (![sliceT uint64T] "config") in
-    do:  "s" <-[ptrT] "$a0";;;
+    let: "$r0" := let: "$a0" := ![stringT] "fname" in
+    let: "$a1" := ![sliceT byteT] "initstate" in
+    let: "$a2" := ![sliceT uint64T] "config" in
+    makeServer "$a0" "$a1" "$a2" in
+    do:  ("s" <-[ptrT] "$r0");;;
     let: "handlers" := ref_ty (mapT uint64T funcT) (zero_val (mapT uint64T funcT)) in
-    let: "$a0" := map.make uint64T funcT #() in
-    do:  "handlers" <-[mapT uint64T funcT] "$a0";;;
-    let: "$a0" := (λ: "raw_args" "raw_reply",
+    let: "$r0" := map.make uint64T funcT #() in
+    do:  ("handlers" <-[mapT uint64T funcT] "$r0");;;
+    let: "$r0" := (λ: "raw_args" "raw_reply",
       let: "reply" := ref_ty ptrT (zero_val ptrT) in
-      let: "$a0" := ref_ty applyAsFollowerReply (zero_val applyAsFollowerReply) in
-      do:  "reply" <-[ptrT] "$a0";;;
+      let: "$r0" := ref_ty applyAsFollowerReply (zero_val applyAsFollowerReply) in
+      do:  ("reply" <-[ptrT] "$r0");;;
       let: "args" := ref_ty ptrT (zero_val ptrT) in
-      let: "$a0" := decodeApplyAsFollowerArgs (![sliceT byteT] "raw_args") in
-      do:  "args" <-[ptrT] "$a0";;;
-      do:  (Server__applyAsFollower (![ptrT] "s")) (![ptrT] "args") (![ptrT] "reply");;;
-      let: "$a0" := encodeApplyAsFollowerReply (![ptrT] "reply") in
-      do:  (![ptrT] "raw_reply") <-[sliceT byteT] "$a0";;;
+      let: "$r0" := let: "$a0" := ![sliceT byteT] "raw_args" in
+      decodeApplyAsFollowerArgs "$a0" in
+      do:  ("args" <-[ptrT] "$r0");;;
+      do:  (let: "$a0" := ![ptrT] "args" in
+      let: "$a1" := ![ptrT] "reply" in
+      (Server__applyAsFollower (![ptrT] "s")) "$a0" "$a1");;;
+      let: "$r0" := let: "$a0" := ![ptrT] "reply" in
+      encodeApplyAsFollowerReply "$a0" in
+      do:  ((![ptrT] "raw_reply") <-[sliceT byteT] "$r0");;;
       do:  #()
       ) in
-    do:  map.insert (![mapT uint64T funcT] "handlers") RPC_APPLY_AS_FOLLOWER "$a0";;;
-    let: "$a0" := (λ: "raw_args" "raw_reply",
+    do:  (map.insert (![mapT uint64T funcT] "handlers") RPC_APPLY_AS_FOLLOWER "$r0");;;
+    let: "$r0" := (λ: "raw_args" "raw_reply",
       let: "reply" := ref_ty ptrT (zero_val ptrT) in
-      let: "$a0" := ref_ty enterNewEpochReply (zero_val enterNewEpochReply) in
-      do:  "reply" <-[ptrT] "$a0";;;
+      let: "$r0" := ref_ty enterNewEpochReply (zero_val enterNewEpochReply) in
+      do:  ("reply" <-[ptrT] "$r0");;;
       let: "args" := ref_ty ptrT (zero_val ptrT) in
-      let: "$a0" := decodeEnterNewEpochArgs (![sliceT byteT] "raw_args") in
-      do:  "args" <-[ptrT] "$a0";;;
-      do:  (Server__enterNewEpoch (![ptrT] "s")) (![ptrT] "args") (![ptrT] "reply");;;
-      let: "$a0" := encodeEnterNewEpochReply (![ptrT] "reply") in
-      do:  (![ptrT] "raw_reply") <-[sliceT byteT] "$a0";;;
+      let: "$r0" := let: "$a0" := ![sliceT byteT] "raw_args" in
+      decodeEnterNewEpochArgs "$a0" in
+      do:  ("args" <-[ptrT] "$r0");;;
+      do:  (let: "$a0" := ![ptrT] "args" in
+      let: "$a1" := ![ptrT] "reply" in
+      (Server__enterNewEpoch (![ptrT] "s")) "$a0" "$a1");;;
+      let: "$r0" := let: "$a0" := ![ptrT] "reply" in
+      encodeEnterNewEpochReply "$a0" in
+      do:  ((![ptrT] "raw_reply") <-[sliceT byteT] "$r0");;;
       do:  #()
       ) in
-    do:  map.insert (![mapT uint64T funcT] "handlers") RPC_ENTER_NEW_EPOCH "$a0";;;
-    let: "$a0" := (λ: "raw_args" "raw_reply",
-      do:  (Server__TryBecomeLeader (![ptrT] "s")) #();;;
+    do:  (map.insert (![mapT uint64T funcT] "handlers") RPC_ENTER_NEW_EPOCH "$r0");;;
+    let: "$r0" := (λ: "raw_args" "raw_reply",
+      do:  ((Server__TryBecomeLeader (![ptrT] "s")) #());;;
       do:  #()
       ) in
-    do:  map.insert (![mapT uint64T funcT] "handlers") RPC_BECOME_LEADER "$a0";;;
+    do:  (map.insert (![mapT uint64T funcT] "handlers") RPC_BECOME_LEADER "$r0");;;
     let: "r" := ref_ty ptrT (zero_val ptrT) in
-    let: "$a0" := urpc.MakeServer (![mapT uint64T funcT] "handlers") in
-    do:  "r" <-[ptrT] "$a0";;;
-    do:  (urpc.Server__Serve (![ptrT] "r")) (![uint64T] "me");;;
+    let: "$r0" := let: "$a0" := ![mapT uint64T funcT] "handlers" in
+    urpc.MakeServer "$a0" in
+    do:  ("r" <-[ptrT] "$r0");;;
+    do:  (let: "$a0" := ![uint64T] "me" in
+    (urpc.Server__Serve (![ptrT] "r")) "$a0");;;
     return: (![ptrT] "s");;;
     do:  #()).
