new/code/github_com/tchajed/marshal.v
@@ -7,80 +7,19 @@ Section code.
 Context `{ffi_syntax}.
 Local Coercion Var' s: expr := Var s.
 
-(* marshal.go *)
-
 Definition Enc : go_type := structT [
   "b" :: sliceT byteT;
   "off" :: ptrT
 ].
 
-Definition NewEncFromSlice : val :=
-  rec: "NewEncFromSlice" "b" :=
-    exception_do (let: "b" := ref_ty (sliceT byteT) "b" in
-    return: (struct.make Enc [{
-       "b" ::= ![sliceT byteT] "b";
-       "off" ::= ref_ty uint64T (zero_val uint64T)
-     }]);;;
-    do:  #()).
-
-Definition NewEnc : val :=
-  rec: "NewEnc" "sz" :=
-    exception_do (let: "sz" := ref_ty uint64T "sz" in
-    let: "b" := ref_ty (sliceT byteT) (zero_val (sliceT byteT)) in
-    let: "$a0" := slice.make2 byteT (![uint64T] "sz") in
-    do:  "b" <-[sliceT byteT] "$a0";;;
-    return: (NewEncFromSlice (![sliceT byteT] "b"));;;
-    do:  #()).
-
-Definition Enc__PutInt : val :=
-  rec: "Enc__PutInt" "enc" "x" :=
+(* go: marshal.go:63:16 *)
+Definition Enc__Finish : val :=
+  rec: "Enc__Finish" "enc" <> :=
     exception_do (let: "enc" := ref_ty Enc "enc" in
-    let: "x" := ref_ty uint64T "x" in
-    let: "off" := ref_ty uint64T (zero_val uint64T) in
-    let: "$a0" := ![uint64T] (![ptrT] (struct.field_ref Enc "off" "enc")) in
-    do:  "off" <-[uint64T] "$a0";;;
-    do:  primitive.UInt64Put (let: "$s" := ![sliceT byteT] (struct.field_ref Enc "b" "enc") in
-    slice.slice byteT "$s" (![uint64T] "off") (slice.len "$s")) (![uint64T] "x");;;
-    do:  (![ptrT] (struct.field_ref Enc "off" "enc")) <-[uint64T] ((![uint64T] (![ptrT] (struct.field_ref Enc "off" "enc"))) + #8);;;
+    return: (![sliceT byteT] (struct.field_ref Enc "b" "enc"));;;
     do:  #()).
 
-Definition Enc__PutInt32 : val :=
-  rec: "Enc__PutInt32" "enc" "x" :=
-    exception_do (let: "enc" := ref_ty Enc "enc" in
-    let: "x" := ref_ty uint32T "x" in
-    let: "off" := ref_ty uint64T (zero_val uint64T) in
-    let: "$a0" := ![uint64T] (![ptrT] (struct.field_ref Enc "off" "enc")) in
-    do:  "off" <-[uint64T] "$a0";;;
-    do:  primitive.UInt32Put (let: "$s" := ![sliceT byteT] (struct.field_ref Enc "b" "enc") in
-    slice.slice byteT "$s" (![uint64T] "off") (slice.len "$s")) (![uint32T] "x");;;
-    do:  (![ptrT] (struct.field_ref Enc "off" "enc")) <-[uint64T] ((![uint64T] (![ptrT] (struct.field_ref Enc "off" "enc"))) + #4);;;
-    do:  #()).
-
-Definition Enc__PutInts : val :=
-  rec: "Enc__PutInts" "enc" "xs" :=
-    exception_do (let: "enc" := ref_ty Enc "enc" in
-    let: "xs" := ref_ty (sliceT uint64T) "xs" in
-    do:  let: "$range" := ![sliceT uint64T] "xs" in
-    slice.for_range uint64T "$range" (λ: <> "x",
-      let: "x" := ref_ty uint64T "x" in
-      do:  (Enc__PutInt (![Enc] "enc")) (![uint64T] "x");;;
-      do:  #());;;
-    do:  #()).
-
-Definition Enc__PutBytes : val :=
-  rec: "Enc__PutBytes" "enc" "b" :=
-    exception_do (let: "enc" := ref_ty Enc "enc" in
-    let: "b" := ref_ty (sliceT byteT) "b" in
-    let: "off" := ref_ty uint64T (zero_val uint64T) in
-    let: "$a0" := ![uint64T] (![ptrT] (struct.field_ref Enc "off" "enc")) in
-    do:  "off" <-[uint64T] "$a0";;;
-    let: "n" := ref_ty uint64T (zero_val uint64T) in
-    let: "$a0" := slice.copy byteT (let: "$s" := ![sliceT byteT] (struct.field_ref Enc "b" "enc") in
-    slice.slice byteT "$s" (![uint64T] "off") (slice.len "$s")) (![sliceT byteT] "b") in
-    do:  "n" <-[uint64T] "$a0";;;
-    do:  (![ptrT] (struct.field_ref Enc "off" "enc")) <-[uint64T] ((![uint64T] (![ptrT] (struct.field_ref Enc "off" "enc"))) + (![uint64T] "n"));;;
-    do:  #()).
-
+(* go: marshal.go:49:6 *)
 Definition bool2byte : val :=
   rec: "bool2byte" "b" :=
     exception_do (let: "b" := ref_ty boolT "b" in
@@ -93,22 +32,115 @@ Definition bool2byte : val :=
       do:  #());;;
     do:  #()).
 
+(* go: marshal.go:57:16 *)
 Definition Enc__PutBool : val :=
   rec: "Enc__PutBool" "enc" "b" :=
     exception_do (let: "enc" := ref_ty Enc "enc" in
     let: "b" := ref_ty boolT "b" in
     let: "off" := ref_ty uint64T (zero_val uint64T) in
-    let: "$a0" := ![uint64T] (![ptrT] (struct.field_ref Enc "off" "enc")) in
-    do:  "off" <-[uint64T] "$a0";;;
-    let: "$a0" := bool2byte (![boolT] "b") in
-    do:  (slice.elem_ref byteT (![sliceT byteT] (struct.field_ref Enc "b" "enc")) (![uint64T] "off")) <-[byteT] "$a0";;;
-    do:  (![ptrT] (struct.field_ref Enc "off" "enc")) <-[uint64T] ((![uint64T] (![ptrT] (struct.field_ref Enc "off" "enc"))) + #1);;;
+    let: "$r0" := ![uint64T] (![ptrT] (struct.field_ref Enc "off" "enc")) in
+    do:  ("off" <-[uint64T] "$r0");;;
+    let: "$r0" := let: "$a0" := ![boolT] "b" in
+    bool2byte "$a0" in
+    do:  ((slice.elem_ref byteT (![sliceT byteT] (struct.field_ref Enc "b" "enc")) (![uint64T] "off")) <-[byteT] "$r0");;;
+    do:  ((![ptrT] (struct.field_ref Enc "off" "enc")) <-[uint64T] ((![uint64T] (![ptrT] (struct.field_ref Enc "off" "enc"))) + #1));;;
     do:  #()).
 
-Definition Enc__Finish : val :=
-  rec: "Enc__Finish" "enc" <> :=
+(* go: marshal.go:43:16 *)
+Definition Enc__PutBytes : val :=
+  rec: "Enc__PutBytes" "enc" "b" :=
     exception_do (let: "enc" := ref_ty Enc "enc" in
-    return: (![sliceT byteT] (struct.field_ref Enc "b" "enc"));;;
+    let: "b" := ref_ty (sliceT byteT) "b" in
+    let: "off" := ref_ty uint64T (zero_val uint64T) in
+    let: "$r0" := ![uint64T] (![ptrT] (struct.field_ref Enc "off" "enc")) in
+    do:  ("off" <-[uint64T] "$r0");;;
+    let: "n" := ref_ty uint64T (zero_val uint64T) in
+    let: "$r0" := slice.copy byteT (let: "$s" := ![sliceT byteT] (struct.field_ref Enc "b" "enc") in
+    slice.slice byteT "$s" (![uint64T] "off") (slice.len "$s")) (![sliceT byteT] "b") in
+    do:  ("n" <-[uint64T] "$r0");;;
+    do:  ((![ptrT] (struct.field_ref Enc "off" "enc")) <-[uint64T] ((![uint64T] (![ptrT] (struct.field_ref Enc "off" "enc"))) + (![uint64T] "n")));;;
+    do:  #()).
+
+(* go: marshal.go:25:16 *)
+Definition Enc__PutInt : val :=
+  rec: "Enc__PutInt" "enc" "x" :=
+    exception_do (let: "enc" := ref_ty Enc "enc" in
+    let: "x" := ref_ty uint64T "x" in
+    let: "off" := ref_ty uint64T (zero_val uint64T) in
+    let: "$r0" := ![uint64T] (![ptrT] (struct.field_ref Enc "off" "enc")) in
+    do:  ("off" <-[uint64T] "$r0");;;
+    do:  (let: "$a0" := let: "$s" := ![sliceT byteT] (struct.field_ref Enc "b" "enc") in
+    slice.slice byteT "$s" (![uint64T] "off") (slice.len "$s") in
+    let: "$a1" := ![uint64T] "x" in
+    primitive.UInt64Put "$a0" "$a1");;;
+    do:  ((![ptrT] (struct.field_ref Enc "off" "enc")) <-[uint64T] ((![uint64T] (![ptrT] (struct.field_ref Enc "off" "enc"))) + #8));;;
+    do:  #()).
+
+(* go: marshal.go:31:16 *)
+Definition Enc__PutInt32 : val :=
+  rec: "Enc__PutInt32" "enc" "x" :=
+    exception_do (let: "enc" := ref_ty Enc "enc" in
+    let: "x" := ref_ty uint32T "x" in
+    let: "off" := ref_ty uint64T (zero_val uint64T) in
+    let: "$r0" := ![uint64T] (![ptrT] (struct.field_ref Enc "off" "enc")) in
+    do:  ("off" <-[uint64T] "$r0");;;
+    do:  (let: "$a0" := let: "$s" := ![sliceT byteT] (struct.field_ref Enc "b" "enc") in
+    slice.slice byteT "$s" (![uint64T] "off") (slice.len "$s") in
+    let: "$a1" := ![uint32T] "x" in
+    primitive.UInt32Put "$a0" "$a1");;;
+    do:  ((![ptrT] (struct.field_ref Enc "off" "enc")) <-[uint64T] ((![uint64T] (![ptrT] (struct.field_ref Enc "off" "enc"))) + #4));;;
+    do:  #()).
+
+(* go: marshal.go:37:16 *)
+Definition Enc__PutInts : val :=
+  rec: "Enc__PutInts" "enc" "xs" :=
+    exception_do (let: "enc" := ref_ty Enc "enc" in
+    let: "xs" := ref_ty (sliceT uint64T) "xs" in
+    do:  (let: "$range" := ![sliceT uint64T] "xs" in
+    slice.for_range uint64T "$range" (λ: <> "x",
+      let: "x" := ref_ty uint64T "x" in
+      do:  (let: "$a0" := ![uint64T] "x" in
+      (Enc__PutInt (![ptrT] "enc")) "$a0");;;
+      do:  #()));;;
+    do:  #()).
+
+Definition Enc__mset : list (string * val) := [
+  ("Finish", Enc__Finish);
+  ("PutBool", Enc__PutBool);
+  ("PutBytes", Enc__PutBytes);
+  ("PutInt", Enc__PutInt);
+  ("PutInt32", Enc__PutInt32);
+  ("PutInts", Enc__PutInts)
+].
+
+Definition Enc__mset_ptr : list (string * val) := [
+  ("Finish", (λ: "r", Enc__Finish (![Enc] "r"))%V);
+  ("PutBool", (λ: "r", Enc__PutBool (![Enc] "r"))%V);
+  ("PutBytes", (λ: "r", Enc__PutBytes (![Enc] "r"))%V);
+  ("PutInt", (λ: "r", Enc__PutInt (![Enc] "r"))%V);
+  ("PutInt32", (λ: "r", Enc__PutInt32 (![Enc] "r"))%V);
+  ("PutInts", (λ: "r", Enc__PutInts (![Enc] "r"))%V)
+].
+
+(* go: marshal.go:13:6 *)
+Definition NewEncFromSlice : val :=
+  rec: "NewEncFromSlice" "b" :=
+    exception_do (let: "b" := ref_ty (sliceT byteT) "b" in
+    return: (struct.make Enc [{
+       "b" ::= ![sliceT byteT] "b";
+       "off" ::= ref_ty uint64T (zero_val uint64T)
+     }]);;;
+    do:  #()).
+
+(* go: marshal.go:20:6 *)
+Definition NewEnc : val :=
+  rec: "NewEnc" "sz" :=
+    exception_do (let: "sz" := ref_ty uint64T "sz" in
+    let: "b" := ref_ty (sliceT byteT) (zero_val (sliceT byteT)) in
+    let: "$r0" := slice.make2 byteT (![uint64T] "sz") in
+    do:  ("b" <-[sliceT byteT] "$r0");;;
+    return: (let: "$a0" := ![sliceT byteT] "b" in
+     NewEncFromSlice "$a0");;;
     do:  #()).
 
 Definition Dec : go_type := structT [
@@ -116,75 +148,14 @@ Definition Dec : go_type := structT [
   "off" :: ptrT
 ].
 
-Definition NewDec : val :=
-  rec: "NewDec" "b" :=
-    exception_do (let: "b" := ref_ty (sliceT byteT) "b" in
-    return: (struct.make Dec [{
-       "b" ::= ![sliceT byteT] "b";
-       "off" ::= ref_ty uint64T (zero_val uint64T)
-     }]);;;
-    do:  #()).
-
-Definition Dec__GetInt : val :=
-  rec: "Dec__GetInt" "dec" <> :=
-    exception_do (let: "dec" := ref_ty Dec "dec" in
-    let: "off" := ref_ty uint64T (zero_val uint64T) in
-    let: "$a0" := ![uint64T] (![ptrT] (struct.field_ref Dec "off" "dec")) in
-    do:  "off" <-[uint64T] "$a0";;;
-    do:  (![ptrT] (struct.field_ref Dec "off" "dec")) <-[uint64T] ((![uint64T] (![ptrT] (struct.field_ref Dec "off" "dec"))) + #8);;;
-    return: (primitive.UInt64Get (let: "$s" := ![sliceT byteT] (struct.field_ref Dec "b" "dec") in
-     slice.slice byteT "$s" (![uint64T] "off") (slice.len "$s")));;;
-    do:  #()).
-
-Definition Dec__GetInt32 : val :=
-  rec: "Dec__GetInt32" "dec" <> :=
-    exception_do (let: "dec" := ref_ty Dec "dec" in
-    let: "off" := ref_ty uint64T (zero_val uint64T) in
-    let: "$a0" := ![uint64T] (![ptrT] (struct.field_ref Dec "off" "dec")) in
-    do:  "off" <-[uint64T] "$a0";;;
-    do:  (![ptrT] (struct.field_ref Dec "off" "dec")) <-[uint64T] ((![uint64T] (![ptrT] (struct.field_ref Dec "off" "dec"))) + #4);;;
-    return: (primitive.UInt32Get (let: "$s" := ![sliceT byteT] (struct.field_ref Dec "b" "dec") in
-     slice.slice byteT "$s" (![uint64T] "off") (slice.len "$s")));;;
-    do:  #()).
-
-Definition Dec__GetInts : val :=
-  rec: "Dec__GetInts" "dec" "num" :=
-    exception_do (let: "dec" := ref_ty Dec "dec" in
-    let: "num" := ref_ty uint64T "num" in
-    let: "xs" := ref_ty (sliceT uint64T) (zero_val (sliceT uint64T)) in
-    (let: "i" := ref_ty uint64T (zero_val uint64T) in
-    let: "$a0" := #0 in
-    do:  "i" <-[uint64T] "$a0";;;
-    (for: (λ: <>, (![uint64T] "i") < (![uint64T] "num")); (λ: <>, do:  "i" <-[uint64T] ((![uint64T] "i") + #1);;;
-    #()) := λ: <>,
-      let: "$a0" := slice.append uint64T (![sliceT uint64T] "xs") (slice.literal uint64T [(Dec__GetInt (![Dec] "dec")) #()]) in
-      do:  "xs" <-[sliceT uint64T] "$a0";;;
-      do:  #()));;;
-    return: (![sliceT uint64T] "xs");;;
-    do:  #()).
-
-Definition Dec__GetBytes : val :=
-  rec: "Dec__GetBytes" "dec" "num" :=
-    exception_do (let: "dec" := ref_ty Dec "dec" in
-    let: "num" := ref_ty uint64T "num" in
-    let: "off" := ref_ty uint64T (zero_val uint64T) in
-    let: "$a0" := ![uint64T] (![ptrT] (struct.field_ref Dec "off" "dec")) in
-    do:  "off" <-[uint64T] "$a0";;;
-    let: "b" := ref_ty (sliceT byteT) (zero_val (sliceT byteT)) in
-    let: "$a0" := let: "$s" := ![sliceT byteT] (struct.field_ref Dec "b" "dec") in
-    slice.slice byteT "$s" (![uint64T] "off") ((![uint64T] "off") + (![uint64T] "num")) in
-    do:  "b" <-[sliceT byteT] "$a0";;;
-    do:  (![ptrT] (struct.field_ref Dec "off" "dec")) <-[uint64T] ((![uint64T] (![ptrT] (struct.field_ref Dec "off" "dec"))) + (![uint64T] "num"));;;
-    return: (![sliceT byteT] "b");;;
-    do:  #()).
-
+(* go: marshal.go:105:16 *)
 Definition Dec__GetBool : val :=
   rec: "Dec__GetBool" "dec" <> :=
     exception_do (let: "dec" := ref_ty Dec "dec" in
     let: "off" := ref_ty uint64T (zero_val uint64T) in
-    let: "$a0" := ![uint64T] (![ptrT] (struct.field_ref Dec "off" "dec")) in
-    do:  "off" <-[uint64T] "$a0";;;
-    do:  (![ptrT] (struct.field_ref Dec "off" "dec")) <-[uint64T] ((![uint64T] (![ptrT] (struct.field_ref Dec "off" "dec"))) + #1);;;
+    let: "$r0" := ![uint64T] (![ptrT] (struct.field_ref Dec "off" "dec")) in
+    do:  ("off" <-[uint64T] "$r0");;;
+    do:  ((![ptrT] (struct.field_ref Dec "off" "dec")) <-[uint64T] ((![uint64T] (![ptrT] (struct.field_ref Dec "off" "dec"))) + #1));;;
     (if: (![byteT] (slice.elem_ref byteT (![sliceT byteT] (struct.field_ref Dec "b" "dec")) (![uint64T] "off"))) = #(U8 0)
     then
       return: (#false);;;
@@ -194,8 +165,92 @@ Definition Dec__GetBool : val :=
       do:  #());;;
     do:  #()).
 
-(* stateless.go *)
+(* go: marshal.go:98:16 *)
+Definition Dec__GetBytes : val :=
+  rec: "Dec__GetBytes" "dec" "num" :=
+    exception_do (let: "dec" := ref_ty Dec "dec" in
+    let: "num" := ref_ty uint64T "num" in
+    let: "off" := ref_ty uint64T (zero_val uint64T) in
+    let: "$r0" := ![uint64T] (![ptrT] (struct.field_ref Dec "off" "dec")) in
+    do:  ("off" <-[uint64T] "$r0");;;
+    let: "b" := ref_ty (sliceT byteT) (zero_val (sliceT byteT)) in
+    let: "$r0" := let: "$s" := ![sliceT byteT] (struct.field_ref Dec "b" "dec") in
+    slice.slice byteT "$s" (![uint64T] "off") ((![uint64T] "off") + (![uint64T] "num")) in
+    do:  ("b" <-[sliceT byteT] "$r0");;;
+    do:  ((![ptrT] (struct.field_ref Dec "off" "dec")) <-[uint64T] ((![uint64T] (![ptrT] (struct.field_ref Dec "off" "dec"))) + (![uint64T] "num")));;;
+    return: (![sliceT byteT] "b");;;
+    do:  #()).
 
+(* go: marshal.go:78:16 *)
+Definition Dec__GetInt : val :=
+  rec: "Dec__GetInt" "dec" <> :=
+    exception_do (let: "dec" := ref_ty Dec "dec" in
+    let: "off" := ref_ty uint64T (zero_val uint64T) in
+    let: "$r0" := ![uint64T] (![ptrT] (struct.field_ref Dec "off" "dec")) in
+    do:  ("off" <-[uint64T] "$r0");;;
+    do:  ((![ptrT] (struct.field_ref Dec "off" "dec")) <-[uint64T] ((![uint64T] (![ptrT] (struct.field_ref Dec "off" "dec"))) + #8));;;
+    return: (let: "$a0" := let: "$s" := ![sliceT byteT] (struct.field_ref Dec "b" "dec") in
+     slice.slice byteT "$s" (![uint64T] "off") (slice.len "$s") in
+     primitive.UInt64Get "$a0");;;
+    do:  #()).
+
+(* go: marshal.go:84:16 *)
+Definition Dec__GetInt32 : val :=
+  rec: "Dec__GetInt32" "dec" <> :=
+    exception_do (let: "dec" := ref_ty Dec "dec" in
+    let: "off" := ref_ty uint64T (zero_val uint64T) in
+    let: "$r0" := ![uint64T] (![ptrT] (struct.field_ref Dec "off" "dec")) in
+    do:  ("off" <-[uint64T] "$r0");;;
+    do:  ((![ptrT] (struct.field_ref Dec "off" "dec")) <-[uint64T] ((![uint64T] (![ptrT] (struct.field_ref Dec "off" "dec"))) + #4));;;
+    return: (let: "$a0" := let: "$s" := ![sliceT byteT] (struct.field_ref Dec "b" "dec") in
+     slice.slice byteT "$s" (![uint64T] "off") (slice.len "$s") in
+     primitive.UInt32Get "$a0");;;
+    do:  #()).
+
+(* go: marshal.go:90:16 *)
+Definition Dec__GetInts : val :=
+  rec: "Dec__GetInts" "dec" "num" :=
+    exception_do (let: "dec" := ref_ty Dec "dec" in
+    let: "num" := ref_ty uint64T "num" in
+    let: "xs" := ref_ty (sliceT uint64T) (zero_val (sliceT uint64T)) in
+    (let: "i" := ref_ty uint64T (zero_val uint64T) in
+    let: "$r0" := #0 in
+    do:  ("i" <-[uint64T] "$r0");;;
+    (for: (λ: <>, (![uint64T] "i") < (![uint64T] "num")); (λ: <>, do:  ("i" <-[uint64T] ((![uint64T] "i") + #1));;;
+    #()) := λ: <>,
+      let: "$r0" := slice.append uint64T (![sliceT uint64T] "xs") (slice.literal uint64T [(Dec__GetInt (![ptrT] "dec")) #()]) in
+      do:  ("xs" <-[sliceT uint64T] "$r0");;;
+      do:  #()));;;
+    return: (![sliceT uint64T] "xs");;;
+    do:  #()).
+
+Definition Dec__mset : list (string * val) := [
+  ("GetBool", Dec__GetBool);
+  ("GetBytes", Dec__GetBytes);
+  ("GetInt", Dec__GetInt);
+  ("GetInt32", Dec__GetInt32);
+  ("GetInts", Dec__GetInts)
+].
+
+Definition Dec__mset_ptr : list (string * val) := [
+  ("GetBool", (λ: "r", Dec__GetBool (![Dec] "r"))%V);
+  ("GetBytes", (λ: "r", Dec__GetBytes (![Dec] "r"))%V);
+  ("GetInt", (λ: "r", Dec__GetInt (![Dec] "r"))%V);
+  ("GetInt32", (λ: "r", Dec__GetInt32 (![Dec] "r"))%V);
+  ("GetInts", (λ: "r", Dec__GetInts (![Dec] "r"))%V)
+].
+
+(* go: marshal.go:74:6 *)
+Definition NewDec : val :=
+  rec: "NewDec" "b" :=
+    exception_do (let: "b" := ref_ty (sliceT byteT) "b" in
+    return: (struct.make Dec [{
+       "b" ::= ![sliceT byteT] "b";
+       "off" ::= ref_ty uint64T (zero_val uint64T)
+     }]);;;
+    do:  #()).
+
+(* go: stateless.go:8:6 *)
 Definition compute_new_cap : val :=
   rec: "compute_new_cap" "old_cap" "min_cap" :=
     exception_do (let: "min_cap" := ref_ty uint64T "min_cap" in
@@ -203,31 +258,37 @@ Definition compute_new_cap : val :=
     let: "new_cap" := ref_ty uint64T ((![uint64T] "old_cap") * #2) in
     (if: (![uint64T] "new_cap") < (![uint64T] "min_cap")
     then
-      let: "$a0" := ![uint64T] "min_cap" in
-      do:  "new_cap" <-[uint64T] "$a0";;;
+      let: "$r0" := ![uint64T] "min_cap" in
+      do:  ("new_cap" <-[uint64T] "$r0");;;
       do:  #()
     else do:  #());;;
     return: (![uint64T] "new_cap");;;
     do:  #()).
 
 (* Grow a slice to have at least `additional` unused bytes in the capacity.
-   Runtime-check against overflow. *)
+   Runtime-check against overflow.
+
+   go: stateless.go:19:6 *)
 Definition reserve : val :=
   rec: "reserve" "b" "additional" :=
     exception_do (let: "additional" := ref_ty uint64T "additional" in
     let: "b" := ref_ty (sliceT byteT) "b" in
     let: "min_cap" := ref_ty uint64T (zero_val uint64T) in
-    let: "$a0" := std.SumAssumeNoOverflow (slice.len (![sliceT byteT] "b")) (![uint64T] "additional") in
-    do:  "min_cap" <-[uint64T] "$a0";;;
+    let: "$r0" := let: "$a0" := slice.len (![sliceT byteT] "b") in
+    let: "$a1" := ![uint64T] "additional" in
+    std.SumAssumeNoOverflow "$a0" "$a1" in
+    do:  ("min_cap" <-[uint64T] "$r0");;;
     (if: (slice.cap (![sliceT byteT] "b")) < (![uint64T] "min_cap")
     then
       let: "new_cap" := ref_ty uint64T (zero_val uint64T) in
-      let: "$a0" := compute_new_cap (slice.cap (![sliceT byteT] "b")) (![uint64T] "min_cap") in
-      do:  "new_cap" <-[uint64T] "$a0";;;
+      let: "$r0" := let: "$a0" := slice.cap (![sliceT byteT] "b") in
+      let: "$a1" := ![uint64T] "min_cap" in
+      compute_new_cap "$a0" "$a1" in
+      do:  ("new_cap" <-[uint64T] "$r0");;;
       let: "dest" := ref_ty (sliceT byteT) (zero_val (sliceT byteT)) in
-      let: "$a0" := slice.make3 byteT (slice.len (![sliceT byteT] "b")) (![uint64T] "new_cap") in
-      do:  "dest" <-[sliceT byteT] "$a0";;;
-      do:  slice.copy byteT (![sliceT byteT] "dest") (![sliceT byteT] "b");;;
+      let: "$r0" := slice.make3 byteT (slice.len (![sliceT byteT] "b")) (![uint64T] "new_cap") in
+      do:  ("dest" <-[sliceT byteT] "$r0");;;
+      do:  (slice.copy byteT (![sliceT byteT] "dest") (![sliceT byteT] "b"));;;
       return: (![sliceT byteT] "dest");;;
       do:  #()
     else
@@ -235,120 +296,151 @@ Definition reserve : val :=
       do:  #());;;
     do:  #()).
 
+(* go: stateless.go:40:6 *)
 Definition ReadInt : val :=
   rec: "ReadInt" "b" :=
     exception_do (let: "b" := ref_ty (sliceT byteT) "b" in
     let: "i" := ref_ty uint64T (zero_val uint64T) in
-    let: "$a0" := primitive.UInt64Get (![sliceT byteT] "b") in
-    do:  "i" <-[uint64T] "$a0";;;
+    let: "$r0" := let: "$a0" := ![sliceT byteT] "b" in
+    primitive.UInt64Get "$a0" in
+    do:  ("i" <-[uint64T] "$r0");;;
     return: (![uint64T] "i", let: "$s" := ![sliceT byteT] "b" in
      slice.slice byteT "$s" #8 (slice.len "$s"));;;
     do:  #()).
 
+(* go: stateless.go:45:6 *)
 Definition ReadInt32 : val :=
   rec: "ReadInt32" "b" :=
     exception_do (let: "b" := ref_ty (sliceT byteT) "b" in
     let: "i" := ref_ty uint32T (zero_val uint32T) in
-    let: "$a0" := primitive.UInt32Get (![sliceT byteT] "b") in
-    do:  "i" <-[uint32T] "$a0";;;
+    let: "$r0" := let: "$a0" := ![sliceT byteT] "b" in
+    primitive.UInt32Get "$a0" in
+    do:  ("i" <-[uint32T] "$r0");;;
     return: (![uint32T] "i", let: "$s" := ![sliceT byteT] "b" in
      slice.slice byteT "$s" #4 (slice.len "$s"));;;
     do:  #()).
 
-(* ReadBytes reads `l` bytes from b and returns (bs, rest) *)
+(* ReadBytes reads `l` bytes from b and returns (bs, rest)
+
+   go: stateless.go:51:6 *)
 Definition ReadBytes : val :=
   rec: "ReadBytes" "b" "l" :=
     exception_do (let: "l" := ref_ty uint64T "l" in
     let: "b" := ref_ty (sliceT byteT) "b" in
     let: "s" := ref_ty (sliceT byteT) (zero_val (sliceT byteT)) in
-    let: "$a0" := let: "$s" := ![sliceT byteT] "b" in
+    let: "$r0" := let: "$s" := ![sliceT byteT] "b" in
     slice.slice byteT "$s" #0 (![uint64T] "l") in
-    do:  "s" <-[sliceT byteT] "$a0";;;
+    do:  ("s" <-[sliceT byteT] "$r0");;;
     return: (![sliceT byteT] "s", let: "$s" := ![sliceT byteT] "b" in
      slice.slice byteT "$s" (![uint64T] "l") (slice.len "$s"));;;
     do:  #()).
 
-(* Like ReadBytes, but avoids keeping the source slice [b] alive. *)
+(* Like ReadBytes, but avoids keeping the source slice [b] alive.
+
+   go: stateless.go:57:6 *)
 Definition ReadBytesCopy : val :=
   rec: "ReadBytesCopy" "b" "l" :=
     exception_do (let: "l" := ref_ty uint64T "l" in
     let: "b" := ref_ty (sliceT byteT) "b" in
     let: "s" := ref_ty (sliceT byteT) (zero_val (sliceT byteT)) in
-    let: "$a0" := slice.make2 byteT (![uint64T] "l") in
-    do:  "s" <-[sliceT byteT] "$a0";;;
-    do:  slice.copy byteT (![sliceT byteT] "s") (let: "$s" := ![sliceT byteT] "b" in
-    slice.slice byteT "$s" #0 (![uint64T] "l"));;;
+    let: "$r0" := slice.make2 byteT (![uint64T] "l") in
+    do:  ("s" <-[sliceT byteT] "$r0");;;
+    do:  (slice.copy byteT (![sliceT byteT] "s") (let: "$s" := ![sliceT byteT] "b" in
+    slice.slice byteT "$s" #0 (![uint64T] "l")));;;
     return: (![sliceT byteT] "s", let: "$s" := ![sliceT byteT] "b" in
      slice.slice byteT "$s" (![uint64T] "l") (slice.len "$s"));;;
     do:  #()).
 
+(* go: stateless.go:63:6 *)
 Definition ReadBool : val :=
   rec: "ReadBool" "b" :=
     exception_do (let: "b" := ref_ty (sliceT byteT) "b" in
     let: "x" := ref_ty boolT (zero_val boolT) in
-    let: "$a0" := (![byteT] (slice.elem_ref byteT (![sliceT byteT] "b") #0)) ≠ #(U8 0) in
-    do:  "x" <-[boolT] "$a0";;;
+    let: "$r0" := (![byteT] (slice.elem_ref byteT (![sliceT byteT] "b") #0)) ≠ #(U8 0) in
+    do:  ("x" <-[boolT] "$r0");;;
     return: (![boolT] "x", let: "$s" := ![sliceT byteT] "b" in
      slice.slice byteT "$s" #1 (slice.len "$s"));;;
     do:  #()).
 
+(* go: stateless.go:68:6 *)
 Definition ReadLenPrefixedBytes : val :=
   rec: "ReadLenPrefixedBytes" "b" :=
     exception_do (let: "b" := ref_ty (sliceT byteT) "b" in
     let: "b2" := ref_ty (sliceT byteT) (zero_val (sliceT byteT)) in
     let: "l" := ref_ty uint64T (zero_val uint64T) in
-    let: ("$a0", "$a1") := ReadInt (![sliceT byteT] "b") in
-    do:  "b2" <-[sliceT byteT] "$a1";;;
-    do:  "l" <-[uint64T] "$a0";;;
+    let: ("$ret0", "$ret1") := let: "$a0" := ![sliceT byteT] "b" in
+    ReadInt "$a0" in
+    let: "$r0" := "$ret0" in
+    let: "$r1" := "$ret1" in
+    do:  ("l" <-[uint64T] "$r0");;;
+    do:  ("b2" <-[sliceT byteT] "$r1");;;
     let: "b3" := ref_ty (sliceT byteT) (zero_val (sliceT byteT)) in
     let: "bs" := ref_ty (sliceT byteT) (zero_val (sliceT byteT)) in
-    let: ("$a0", "$a1") := ReadBytes (![sliceT byteT] "b2") (![uint64T] "l") in
-    do:  "b3" <-[sliceT byteT] "$a1";;;
-    do:  "bs" <-[sliceT byteT] "$a0";;;
+    let: ("$ret0", "$ret1") := let: "$a0" := ![sliceT byteT] "b2" in
+    let: "$a1" := ![uint64T] "l" in
+    ReadBytes "$a0" "$a1" in
+    let: "$r0" := "$ret0" in
+    let: "$r1" := "$ret1" in
+    do:  ("bs" <-[sliceT byteT] "$r0");;;
+    do:  ("b3" <-[sliceT byteT] "$r1");;;
     return: (![sliceT byteT] "bs", ![sliceT byteT] "b3");;;
     do:  #()).
 
-(* WriteInt appends i in little-endian format to b, returning the new slice. *)
+(* WriteInt appends i in little-endian format to b, returning the new slice.
+
+   go: stateless.go:77:6 *)
 Definition WriteInt : val :=
   rec: "WriteInt" "b" "i" :=
     exception_do (let: "i" := ref_ty uint64T "i" in
     let: "b" := ref_ty (sliceT byteT) "b" in
     let: "b2" := ref_ty (sliceT byteT) (zero_val (sliceT byteT)) in
-    let: "$a0" := reserve (![sliceT byteT] "b") #8 in
-    do:  "b2" <-[sliceT byteT] "$a0";;;
+    let: "$r0" := let: "$a0" := ![sliceT byteT] "b" in
+    let: "$a1" := #8 in
+    reserve "$a0" "$a1" in
+    do:  ("b2" <-[sliceT byteT] "$r0");;;
     let: "off" := ref_ty intT (zero_val intT) in
-    let: "$a0" := slice.len (![sliceT byteT] "b2") in
-    do:  "off" <-[intT] "$a0";;;
+    let: "$r0" := slice.len (![sliceT byteT] "b2") in
+    do:  ("off" <-[intT] "$r0");;;
     let: "b3" := ref_ty (sliceT byteT) (zero_val (sliceT byteT)) in
-    let: "$a0" := let: "$s" := ![sliceT byteT] "b2" in
+    let: "$r0" := let: "$s" := ![sliceT byteT] "b2" in
     slice.slice byteT "$s" #0 ((![intT] "off") + #8) in
-    do:  "b3" <-[sliceT byteT] "$a0";;;
-    do:  primitive.UInt64Put (let: "$s" := ![sliceT byteT] "b3" in
-    slice.slice byteT "$s" (![intT] "off") (slice.len "$s")) (![uint64T] "i");;;
+    do:  ("b3" <-[sliceT byteT] "$r0");;;
+    do:  (let: "$a0" := let: "$s" := ![sliceT byteT] "b3" in
+    slice.slice byteT "$s" (![intT] "off") (slice.len "$s") in
+    let: "$a1" := ![uint64T] "i" in
+    primitive.UInt64Put "$a0" "$a1");;;
     return: (![sliceT byteT] "b3");;;
     do:  #()).
 
-(* WriteInt32 appends 32-bit integer i in little-endian format to b, returning the new slice. *)
+(* WriteInt32 appends 32-bit integer i in little-endian format to b, returning the new slice.
+
+   go: stateless.go:87:6 *)
 Definition WriteInt32 : val :=
   rec: "WriteInt32" "b" "i" :=
     exception_do (let: "i" := ref_ty uint32T "i" in
     let: "b" := ref_ty (sliceT byteT) "b" in
     let: "b2" := ref_ty (sliceT byteT) (zero_val (sliceT byteT)) in
-    let: "$a0" := reserve (![sliceT byteT] "b") #4 in
-    do:  "b2" <-[sliceT byteT] "$a0";;;
+    let: "$r0" := let: "$a0" := ![sliceT byteT] "b" in
+    let: "$a1" := #4 in
+    reserve "$a0" "$a1" in
+    do:  ("b2" <-[sliceT byteT] "$r0");;;
     let: "off" := ref_ty intT (zero_val intT) in
-    let: "$a0" := slice.len (![sliceT byteT] "b2") in
-    do:  "off" <-[intT] "$a0";;;
+    let: "$r0" := slice.len (![sliceT byteT] "b2") in
+    do:  ("off" <-[intT] "$r0");;;
     let: "b3" := ref_ty (sliceT byteT) (zero_val (sliceT byteT)) in
-    let: "$a0" := let: "$s" := ![sliceT byteT] "b2" in
+    let: "$r0" := let: "$s" := ![sliceT byteT] "b2" in
     slice.slice byteT "$s" #0 ((![intT] "off") + #4) in
-    do:  "b3" <-[sliceT byteT] "$a0";;;
-    do:  primitive.UInt32Put (let: "$s" := ![sliceT byteT] "b3" in
-    slice.slice byteT "$s" (![intT] "off") (slice.len "$s")) (![uint32T] "i");;;
+    do:  ("b3" <-[sliceT byteT] "$r0");;;
+    do:  (let: "$a0" := let: "$s" := ![sliceT byteT] "b3" in
+    slice.slice byteT "$s" (![intT] "off") (slice.len "$s") in
+    let: "$a1" := ![uint32T] "i" in
+    primitive.UInt32Put "$a0" "$a1");;;
     return: (![sliceT byteT] "b3");;;
     do:  #()).
 
-(* Append data to b, returning the new slice. *)
+(* Append data to b, returning the new slice.
+
+   go: stateless.go:96:6 *)
 Definition WriteBytes : val :=
   rec: "WriteBytes" "b" "data" :=
     exception_do (let: "data" := ref_ty (sliceT byteT) "data" in
@@ -356,6 +448,7 @@ Definition WriteBytes : val :=
     return: (slice.append byteT (![sliceT byteT] "b") (![sliceT byteT] "data"));;;
     do:  #()).
 
+(* go: stateless.go:100:6 *)
 Definition WriteBool : val :=
   rec: "WriteBool" "b" "x" :=
     exception_do (let: "x" := ref_ty boolT "x" in
@@ -369,14 +462,19 @@ Definition WriteBool : val :=
       do:  #());;;
     do:  #()).
 
+(* go: stateless.go:108:6 *)
 Definition WriteLenPrefixedBytes : val :=
   rec: "WriteLenPrefixedBytes" "b" "bs" :=
     exception_do (let: "bs" := ref_ty (sliceT byteT) "bs" in
     let: "b" := ref_ty (sliceT byteT) "b" in
     let: "b2" := ref_ty (sliceT byteT) (zero_val (sliceT byteT)) in
-    let: "$a0" := WriteInt (![sliceT byteT] "b") (slice.len (![sliceT byteT] "bs")) in
-    do:  "b2" <-[sliceT byteT] "$a0";;;
-    return: (WriteBytes (![sliceT byteT] "b2") (![sliceT byteT] "bs"));;;
+    let: "$r0" := let: "$a0" := ![sliceT byteT] "b" in
+    let: "$a1" := slice.len (![sliceT byteT] "bs") in
+    WriteInt "$a0" "$a1" in
+    do:  ("b2" <-[sliceT byteT] "$r0");;;
+    return: (let: "$a0" := ![sliceT byteT] "b2" in
+     let: "$a1" := ![sliceT byteT] "bs" in
+     WriteBytes "$a0" "$a1");;;
     do:  #()).
 
 End code.
