new/golang/defn.v
@@ -1,3 +1,3 @@
 From Perennial.goose_lang Require Export lang notation.
-From New.golang.defn Require Export exception list typing noop loop struct mem slice map.
+From New.golang.defn Require Export exception list typing noop loop struct mem slice map interface.
 Open Scope struct_scope.
