new/golang/theory/interface.v
@@ -1,12 +1,26 @@
-From Perennial.goose_lang Require Import notation.
+From Perennial.goose_lang Require Import notation proofmode.
+From New.golang.theory Require Import struct typing.
 From New.golang.defn Require Import interface.
 
-Section pure_execs.
-Context `{ffi_sem: ffi_semantics}.
+Section wps.
+Context `{sem: ffi_semantics} `{!ffi_interp ffi} `{!heapGS Σ}.
 
-Global Instance pure_interface_call (iv : gmap string val) (name : string) (m : val) :
-  WpPureExec (iv !! name = Some m) 2 (interface.call (interface.val iv) #(str name)) m.
+Global Instance wp__interface_get (v : val) (mset : list (string * val)) (method : string) :
+  PureWp (True) (interface.get method (interface.val mset v))
+    (match (assocl_lookup method mset) with | None => (App #() v) | Some m => (App m v) end).
 Proof.
-Admitted.
+  iIntros (?????) "Hwp".
+  rewrite interface.val_unseal.
+  wp_rec. wp_pures.
+  destruct (assocl_lookup method mset); wp_pures; done.
+Qed.
 
-End pure_execs.
+Global Instance wp_interface_make (v : val) (mset : list (string * val)) :
+  PureWp (True) (interface.make mset v) (interface.val mset v).
+Proof.
+  iIntros (?????) "Hwp".
+  rewrite interface.val_unseal interface.make_unseal.
+  wp_rec. wp_pures. done.
+Qed.
+
+End wps.
